db_client helpers

verif/indices/client/db_client.c
@@ -1,58 +1,62 @@
 #include "db_client.h"
 #include "relation.h"
+#include "relation_mem.c"
 #include <stdlib.h>
 #include <stddef.h>
 #include <string.h>
 #include <stdio.h>
+#include "assert.h"
 
 // init all btree methods
-void* btree_create_index () {
-    return RL_NewRelation();
+DB_Cursor_T btree_create_index () {
+    return (DB_Cursor_T) RL_NewRelation();
 }
 
-void* btree_create_cursor (void* env) {
+DB_Cursor_T btree_create_cursor (Index_T env) {
     Relation_T tree = (Relation_T) env;
     BtreeCursor_T cursor = malloc(sizeof(struct BtreeCursor));
+    assert(cursor != NULL);
     cursor->btree = tree;
     cursor->cur = RL_NewCursor(tree);
-    return cursor;
+    return (DB_Cursor_T) cursor;
 }
 
-size_t btree_cardinality (void* env) {
+size_t btree_cardinality (DB_Cursor_T env) {
     BtreeCursor_T cursor = (BtreeCursor_T) env;
     return RL_NumRecords(cursor->cur);
 }
 
-Bool btree_move_to_next (void* env) {
+Bool btree_move_to_next (DB_Cursor_T env) {
     BtreeCursor_T cursor = (BtreeCursor_T) env;
     return RL_MoveToNextValid(cursor->cur);
 }
 
-Bool btree_move_to_first (void* env) {
+Bool btree_move_to_first (DB_Cursor_T env) {
     BtreeCursor_T cursor = (BtreeCursor_T) env;
     return RL_MoveToFirst(cursor->cur);
 }
 
-void* btree_go_to_key (void* env, entry key) {
+Bool btree_go_to_key (DB_Cursor_T env, Key_T key) {
     BtreeCursor_T cursor = (BtreeCursor_T) env;
-    RL_MoveToKey(cursor->cur, (key.cont).int_cont);
-    return cursor;
+    entry* k = (entry*) key;
+    goToKey(cursor->cur, k->int_cont);
+    return RL_CursorIsValid(cursor->cur);
 }
 
-Bool btree_cursor_has_next (void* env) {
+Bool btree_cursor_has_next (DB_Cursor_T env) {
     BtreeCursor_T cursor = (BtreeCursor_T) env;
     return RL_CursorIsValid(cursor->cur);
 }
 
-void* btree_put_record (void* env, entry key, const void* value) {
+void btree_put_record (DB_Cursor_T env, Key_T key, const Value_T value) {
     BtreeCursor_T cursor = (BtreeCursor_T) env;
-    RL_PutRecord(cursor->cur, (key.cont).int_cont, value);
-    return cursor;
+    entry* k = (entry*) key;
+    RL_PutRecord(cursor->cur, k->int_cont, value);
 }
 
-const void* btree_get_record (void* env) {
+const Value_T btree_get_record (DB_Cursor_T env) {
     BtreeCursor_T cursor = (BtreeCursor_T) env;
-    return RL_GetRecord(cursor->cur);
+    return (Value_T) RL_GetRecord(cursor->cur);
 }
 
 OrdIndexMtable btree_mtable =
@@ -73,8 +77,8 @@ size_t attr_list_length(attribute_list_t lst) {
 
 // for now, assumes only 1 pk column
 // return -1 if no match
-size_t index_of_pk_column(attribute_list_t lst, attribute_list_t pk) {
-    size_t ind = 0;
+int index_of_pk_column(attribute_list_t lst, attribute_list_t pk) {
+    int ind = 0;
     char* pk_ID = pk->id;
     while(lst != NULL) {
         if (strcmp(pk_ID, lst->id) == 0) {
@@ -86,54 +90,51 @@ size_t index_of_pk_column(attribute_list_t lst, attribute_list_t pk) {
     return -1;
 }
 
-Relation_T create_relation(entry arr[], size_t numrows, index_attributes_t att) {
-    
-    // if our key is not integer, return null
-    if (att->pk_attrs->domain != Int) {
-        return NULL;
-    }
-    
+Cursor_T malloc_btree_cursor() {
     Relation_T rel = RL_NewRelation();
     Cursor_T cur = RL_NewCursor(rel);
+    return cur;
+}
+
+Relation_T fill_relation(entry arr[], Cursor_T cur, size_t numrows, index_attributes_t att) {
     size_t numcols = attr_list_length(att->attrs);
     size_t pk_num = index_of_pk_column(att->attrs, att->pk_attrs);
-    
     size_t i;
     for (i = 0; i < numrows; i++) {
         void* ptr_to_row = &arr[i * numcols];
         entry key = arr[i*numcols + pk_num];
-        RL_PutRecord(cur, (key.cont).int_cont, ptr_to_row);
+        RL_PutRecord(cur, key.int_cont, ptr_to_row);
     }
-    
-    return rel;
+    return cur->relation;
 }
 
+// data - 2 columns, student id and name
+entry data[] = {{ .int_cont = 1}, { .str_cont = "Alice"},
+                { .int_cont = 2}, { .str_cont = "Bob"},
+                { .int_cont = 3}, { .str_cont = "Claire"},
+                { .int_cont = 4}, { .str_cont = "Dean"}};
+
+// two columns, student ID and student Name
+struct attribute_list snd = {"Name", Str, NULL};
+struct attribute_list schema = {"ID", Int, &snd};
+// the primary key is just the ID column
+struct attribute_list primary = {"ID", Int, NULL};
+// index attrs
+struct index_attributes attrs = {&schema, &primary};
+
+
+
 int main(int argc, char *argv[]) {
-    entry e1 = {Int, { .int_cont = 1}};
-    entry e2 = {Str, { .str_cont = "Alice"}};
-    entry e3 = {Int, { .int_cont = 2}};
-    entry e4 = {Str, { .str_cont = "Bob"}};
-    entry e5 = {Int, { .int_cont = 3}};
-    entry e6 = {Str, { .str_cont = "Claire"}};
-    entry e7 = {Int, { .int_cont = 4}};
-    entry e8 = {Str, { .str_cont = "Dean"}};
-    entry data[] = {e1, e2, e3, e4, e5, e6, e7, e8};
     
-    // two columns, student ID and student Name
-    struct attribute_list snd = {"Name", Str, NULL};
-    struct attribute_list schema = {"ID", Int, &snd};
-    // the primary key is just the ID column
-    struct attribute_list primary = {"ID", Int, NULL};
-    // index attrs
-    struct index_attributes attrs = {&schema, &primary};
+    Cursor_T cur = malloc_btree_cursor();
+    Index_T tree = (Index_T) fill_relation(data, cur, 4, &attrs);
     
-    Relation_T tree = create_relation(data, 4, &attrs);
     
     // first cursor
-    BtreeCursor_T bc1 = (BtreeCursor_T) btree_mtable.create_cursor(tree);
+    DB_Cursor_T bc1 = (DB_Cursor_T) btree_mtable.create_cursor(tree);
     
     // second cursor
-    BtreeCursor_T bc2 = (BtreeCursor_T) btree_mtable.create_cursor(tree);
+    DB_Cursor_T bc2 = (DB_Cursor_T) btree_mtable.create_cursor(tree);
     
     // move the first cursor once
     btree_mtable.move_to_next(bc1);
@@ -141,14 +142,14 @@ int main(int argc, char *argv[]) {
     btree_mtable.move_to_next(bc2);
     btree_mtable.move_to_next(bc2);
     
-    const entry* rec1 = (const entry*) btree_mtable.get_record(bc1);
-    const entry* rec2 = (const entry*) btree_mtable.get_record(bc2);
+  /*  const entry_t* rec1 = (const entry_t*) btree_mtable.get_record(bc1);
+    const entry_t* rec2 = (const entry_t*) btree_mtable.get_record(bc2);
     
-    size_t id1 = ((*rec1).cont).int_cont;
-    char* name1 = (*(rec1 + 1)).cont.str_cont;
-    size_t id2 = ((*rec2).cont).int_cont;
-    char* name2 = (*(rec2 + 1)).cont.str_cont;
+    size_t id1 = ((*rec1)->cont).int_cont;
+    char* name1 = ((*(rec1 + 1))->cont).str_cont;
+    size_t id2 = ((*rec2)->cont).int_cont;
+    char* name2 = ((*(rec2 + 1)))->cont.str_cont;
     
     printf("ID: %d, Name: %s \n", (int) id1, name1);
-    printf("ID: %d, Name: %s \n", (int) id2, name2);
+    printf("ID: %d, Name: %s \n", (int) id2, name2); */
 }
