verif/indices/db_client.v
@@ -11,17 +11,19 @@ Module Info.
   Definition abi := "macosx"%string.
   Definition bitsize := 64.
   Definition big_endian := false.
-  Definition source_file := "relation_mem.c"%string.
+  Definition source_file := "db_client.c"%string.
   Definition normalized := true.
 End Info.
 
 Definition _AscendToParent : ident := 142%positive.
 Definition _BtNode : ident := 26%positive.
+Definition _BtreeCursor : ident := 203%positive.
 Definition _Child_or_Record : ident := 33%positive.
 Definition _Cursor : ident := 47%positive.
 Definition _Entry : ident := 36%positive.
 Definition _First : ident := 38%positive.
 Definition _Last : ident := 39%positive.
+Definition _OrdIndexMtable : ident := 217%positive.
 Definition _RL_CursorIsValid : ident := 130%positive.
 Definition _RL_DeleteRecord : ident := 150%positive.
 Definition _RL_DeleteRelation : ident := 123%positive.
@@ -112,6 +114,13 @@ Definition ___stringlit_2 : ident := 120%positive.
 Definition ___stringlit_20 : ident := 188%positive.
 Definition ___stringlit_21 : ident := 189%positive.
 Definition ___stringlit_22 : ident := 190%positive.
+Definition ___stringlit_23 : ident := 223%positive.
+Definition ___stringlit_24 : ident := 252%positive.
+Definition ___stringlit_25 : ident := 253%positive.
+Definition ___stringlit_26 : ident := 254%positive.
+Definition ___stringlit_27 : ident := 255%positive.
+Definition ___stringlit_28 : ident := 257%positive.
+Definition ___stringlit_29 : ident := 259%positive.
 Definition ___stringlit_3 : ident := 121%positive.
 Definition ___stringlit_4 : ident := 129%positive.
 Definition ___stringlit_5 : ident := 143%positive.
@@ -145,38 +154,82 @@ Definition _abort : ident := 99%positive.
 Definition _allEntries : ident := 169%positive.
 Definition _ancestors : ident := 46%positive.
 Definition _ancestorsIdx : ident := 45%positive.
+Definition _argc : ident := 261%positive.
+Definition _argv : ident := 262%positive.
+Definition _arr : ident := 245%positive.
+Definition _att : ident := 242%positive.
+Definition _attr_list_length : ident := 237%positive.
+Definition _attribute_list : ident := 194%positive.
+Definition _attrs : ident := 196%positive.
+Definition _bc1 : ident := 263%positive.
+Definition _bc2 : ident := 264%positive.
 Definition _btCursor : ident := 127%positive.
+Definition _btree : ident := 201%positive.
+Definition _btree_cardinality : ident := 225%positive.
+Definition _btree_create_cursor : ident := 224%positive.
+Definition _btree_create_index : ident := 220%positive.
+Definition _btree_cursor_has_next : ident := 230%positive.
+Definition _btree_get_record : ident := 233%positive.
+Definition _btree_go_to_key : ident := 229%positive.
+Definition _btree_move_to_first : ident := 227%positive.
+Definition _btree_move_to_next : ident := 226%positive.
+Definition _btree_mtable : ident := 234%positive.
+Definition _btree_put_record : ident := 232%positive.
+Definition _cardinality : ident := 208%positive.
 Definition _child : ident := 31%positive.
 Definition _createNewNode : ident := 116%positive.
+Definition _create_cursor : ident := 207%positive.
+Definition _create_index : ident := 205%positive.
+Definition _create_relation : ident := 244%positive.
+Definition _cur : ident := 202%positive.
 Definition _currNode : ident := 111%positive.
 Definition _currNode__1 : ident := 174%positive.
 Definition _cursor : ident := 109%positive.
+Definition _cursor_has_next : ident := 213%positive.
+Definition _data : ident := 251%positive.
+Definition _db_cursor_t : ident := 204%positive.
 Definition _depth : ident := 29%positive.
+Definition _domain : ident := 193%positive.
 Definition _e : ident := 180%positive.
 Definition _entries : ident := 42%positive.
 Definition _entry : ident := 168%positive.
 Definition _entryIndex : ident := 110%positive.
+Definition _entry__2 : ident := 219%positive.
+Definition _env : ident := 221%positive.
 Definition _exit : ident := 105%positive.
+Definition _fill_relation : ident := 250%positive.
 Definition _findChildIndex : ident := 140%positive.
 Definition _findRecordIndex : ident := 171%positive.
 Definition _firstpointer : ident := 154%positive.
 Definition _fprintf : ident := 101%positive.
 Definition _free : ident := 103%positive.
 Definition _freeRecord : ident := 118%positive.
+Definition _get_record : ident := 216%positive.
 Definition _goToKey : ident := 132%positive.
+Definition _go_to_key : ident := 212%positive.
 Definition _handleDeleteBtree : ident := 122%positive.
 Definition _highest : ident := 139%positive.
 Definition _i : ident := 124%positive.
 Definition _i__1 : ident := 176%positive.
+Definition _id : ident := 192%positive.
 Definition _idx : ident := 137%positive.
+Definition _ind : ident := 239%positive.
+Definition _index_attributes : ident := 198%positive.
+Definition _index_of_pk_column : ident := 241%positive.
+Definition _index_t : ident := 206%positive.
+Definition _int_cont : ident := 199%positive.
 Definition _isFirst : ident := 113%positive.
 Definition _isLeaf : ident := 37%positive.
 Definition _isNodeParent : ident := 141%positive.
 Definition _isValid : ident := 112%positive.
+Definition _k : ident := 228%positive.
 Definition _key : ident := 34%positive.
+Definition _key_t : ident := 211%positive.
 Definition _lastpointer : ident := 153%positive.
+Definition _length : ident := 236%positive.
 Definition _level : ident := 44%positive.
 Definition _lowest : ident := 138%positive.
+Definition _lst : ident := 235%positive.
 Definition _main : ident := 191%positive.
 Definition _malloc : ident := 104%positive.
 Definition _moveToFirst : ident := 125%positive.
@@ -184,99 +237,119 @@ Definition _moveToKey : ident := 148%positive.
 Definition _moveToLast : ident := 155%positive.
 Definition _moveToNext : ident := 144%positive.
 Definition _moveToPrev : ident := 156%positive.
+Definition _move_to_first : ident := 210%positive.
+Definition _move_to_next : ident := 209%positive.
 Definition _n : ident := 106%positive.
 Definition _newEntry : ident := 131%positive.
 Definition _newNode : ident := 167%positive.
+Definition _next : ident := 195%positive.
 Definition _node : ident := 136%positive.
 Definition _numKeys : ident := 40%positive.
 Definition _numRecords : ident := 28%positive.
+Definition _numcols : ident := 247%positive.
+Definition _numrows : ident := 246%positive.
 Definition _p : ident := 107%positive.
 Definition _pNewRelation : ident := 115%positive.
 Definition _pRootNode : ident := 114%positive.
+Definition _pk : ident := 238%positive.
+Definition _pk_ID : ident := 240%positive.
+Definition _pk_attrs : ident := 197%positive.
+Definition _pk_num : ident := 248%positive.
+Definition _primary : ident := 260%positive.
 Definition _printCursor : ident := 165%positive.
 Definition _printTree : ident := 163%positive.
 Definition _printf : ident := 102%positive.
 Definition _ptr : ident := 35%positive.
 Definition _ptr0 : ident := 41%positive.
+Definition _ptr_to_row : ident := 249%positive.
 Definition _putEntry : ident := 133%positive.
+Definition _put_record : ident := 215%positive.
 Definition _record : ident := 32%positive.
+Definition _rel : ident := 243%positive.
 Definition _relation : ident := 43%positive.
 Definition _root : ident := 27%positive.
+Definition _schema : ident := 258%positive.
+Definition _snd : ident := 256%positive.
 Definition _splitnode : ident := 173%positive.
+Definition _str_cont : ident := 200%positive.
+Definition _strcmp : ident := 218%positive.
 Definition _surely_malloc : ident := 108%positive.
 Definition _tgtIdx : ident := 170%positive.
 Definition _tgtIdx__1 : ident := 175%positive.
-Definition _t'1 : ident := 192%positive.
-Definition _t'10 : ident := 201%positive.
-Definition _t'11 : ident := 202%positive.
-Definition _t'12 : ident := 203%positive.
-Definition _t'13 : ident := 204%positive.
-Definition _t'14 : ident := 205%positive.
-Definition _t'15 : ident := 206%positive.
-Definition _t'16 : ident := 207%positive.
-Definition _t'17 : ident := 208%positive.
-Definition _t'18 : ident := 209%positive.
-Definition _t'19 : ident := 210%positive.
-Definition _t'2 : ident := 193%positive.
-Definition _t'20 : ident := 211%positive.
-Definition _t'21 : ident := 212%positive.
-Definition _t'22 : ident := 213%positive.
-Definition _t'23 : ident := 214%positive.
-Definition _t'24 : ident := 215%positive.
-Definition _t'25 : ident := 216%positive.
-Definition _t'26 : ident := 217%positive.
-Definition _t'27 : ident := 218%positive.
-Definition _t'28 : ident := 219%positive.
-Definition _t'29 : ident := 220%positive.
-Definition _t'3 : ident := 194%positive.
-Definition _t'30 : ident := 221%positive.
-Definition _t'31 : ident := 222%positive.
-Definition _t'32 : ident := 223%positive.
-Definition _t'33 : ident := 224%positive.
-Definition _t'34 : ident := 225%positive.
-Definition _t'35 : ident := 226%positive.
-Definition _t'36 : ident := 227%positive.
-Definition _t'37 : ident := 228%positive.
-Definition _t'38 : ident := 229%positive.
-Definition _t'39 : ident := 230%positive.
-Definition _t'4 : ident := 195%positive.
-Definition _t'40 : ident := 231%positive.
-Definition _t'41 : ident := 232%positive.
-Definition _t'42 : ident := 233%positive.
-Definition _t'43 : ident := 234%positive.
-Definition _t'44 : ident := 235%positive.
-Definition _t'45 : ident := 236%positive.
-Definition _t'46 : ident := 237%positive.
-Definition _t'47 : ident := 238%positive.
-Definition _t'48 : ident := 239%positive.
-Definition _t'49 : ident := 240%positive.
-Definition _t'5 : ident := 196%positive.
-Definition _t'50 : ident := 241%positive.
-Definition _t'51 : ident := 242%positive.
-Definition _t'52 : ident := 243%positive.
-Definition _t'53 : ident := 244%positive.
-Definition _t'54 : ident := 245%positive.
-Definition _t'55 : ident := 246%positive.
-Definition _t'56 : ident := 247%positive.
-Definition _t'57 : ident := 248%positive.
-Definition _t'58 : ident := 249%positive.
-Definition _t'59 : ident := 250%positive.
-Definition _t'6 : ident := 197%positive.
-Definition _t'60 : ident := 251%positive.
-Definition _t'61 : ident := 252%positive.
-Definition _t'62 : ident := 253%positive.
-Definition _t'63 : ident := 254%positive.
-Definition _t'64 : ident := 255%positive.
-Definition _t'65 : ident := 256%positive.
-Definition _t'66 : ident := 257%positive.
-Definition _t'67 : ident := 258%positive.
-Definition _t'68 : ident := 259%positive.
-Definition _t'69 : ident := 260%positive.
-Definition _t'7 : ident := 198%positive.
-Definition _t'70 : ident := 261%positive.
-Definition _t'71 : ident := 262%positive.
-Definition _t'8 : ident := 199%positive.
-Definition _t'9 : ident := 200%positive.
+Definition _tree : ident := 222%positive.
+Definition _value : ident := 231%positive.
+Definition _value_t : ident := 214%positive.
+Definition _t'1 : ident := 265%positive.
+Definition _t'10 : ident := 274%positive.
+Definition _t'11 : ident := 275%positive.
+Definition _t'12 : ident := 276%positive.
+Definition _t'13 : ident := 277%positive.
+Definition _t'14 : ident := 278%positive.
+Definition _t'15 : ident := 279%positive.
+Definition _t'16 : ident := 280%positive.
+Definition _t'17 : ident := 281%positive.
+Definition _t'18 : ident := 282%positive.
+Definition _t'19 : ident := 283%positive.
+Definition _t'2 : ident := 266%positive.
+Definition _t'20 : ident := 284%positive.
+Definition _t'21 : ident := 285%positive.
+Definition _t'22 : ident := 286%positive.
+Definition _t'23 : ident := 287%positive.
+Definition _t'24 : ident := 288%positive.
+Definition _t'25 : ident := 289%positive.
+Definition _t'26 : ident := 290%positive.
+Definition _t'27 : ident := 291%positive.
+Definition _t'28 : ident := 292%positive.
+Definition _t'29 : ident := 293%positive.
+Definition _t'3 : ident := 267%positive.
+Definition _t'30 : ident := 294%positive.
+Definition _t'31 : ident := 295%positive.
+Definition _t'32 : ident := 296%positive.
+Definition _t'33 : ident := 297%positive.
+Definition _t'34 : ident := 298%positive.
+Definition _t'35 : ident := 299%positive.
+Definition _t'36 : ident := 300%positive.
+Definition _t'37 : ident := 301%positive.
+Definition _t'38 : ident := 302%positive.
+Definition _t'39 : ident := 303%positive.
+Definition _t'4 : ident := 268%positive.
+Definition _t'40 : ident := 304%positive.
+Definition _t'41 : ident := 305%positive.
+Definition _t'42 : ident := 306%positive.
+Definition _t'43 : ident := 307%positive.
+Definition _t'44 : ident := 308%positive.
+Definition _t'45 : ident := 309%positive.
+Definition _t'46 : ident := 310%positive.
+Definition _t'47 : ident := 311%positive.
+Definition _t'48 : ident := 312%positive.
+Definition _t'49 : ident := 313%positive.
+Definition _t'5 : ident := 269%positive.
+Definition _t'50 : ident := 314%positive.
+Definition _t'51 : ident := 315%positive.
+Definition _t'52 : ident := 316%positive.
+Definition _t'53 : ident := 317%positive.
+Definition _t'54 : ident := 318%positive.
+Definition _t'55 : ident := 319%positive.
+Definition _t'56 : ident := 320%positive.
+Definition _t'57 : ident := 321%positive.
+Definition _t'58 : ident := 322%positive.
+Definition _t'59 : ident := 323%positive.
+Definition _t'6 : ident := 270%positive.
+Definition _t'60 : ident := 324%positive.
+Definition _t'61 : ident := 325%positive.
+Definition _t'62 : ident := 326%positive.
+Definition _t'63 : ident := 327%positive.
+Definition _t'64 : ident := 328%positive.
+Definition _t'65 : ident := 329%positive.
+Definition _t'66 : ident := 330%positive.
+Definition _t'67 : ident := 331%positive.
+Definition _t'68 : ident := 332%positive.
+Definition _t'69 : ident := 333%positive.
+Definition _t'7 : ident := 271%positive.
+Definition _t'70 : ident := 334%positive.
+Definition _t'71 : ident := 335%positive.
+Definition _t'8 : ident := 272%positive.
+Definition _t'9 : ident := 273%positive.
 
 Definition v___stringlit_14 := {|
   gvar_info := (tarray tschar 11);
@@ -300,6 +373,34 @@ Definition v___stringlit_4 := {|
                 Init_int8 (Int.repr 78) :: Init_int8 (Int.repr 85) ::
                 Init_int8 (Int.repr 76) :: Init_int8 (Int.repr 76) ::
                 Init_int8 (Int.repr 0) :: nil);
+  gvar_readonly := true;
+  gvar_volatile := false
+|}.
+
+Definition v___stringlit_23 := {|
+  gvar_info := (tarray tschar 12);
+  gvar_init := (Init_int8 (Int.repr 100) :: Init_int8 (Int.repr 98) ::
+                Init_int8 (Int.repr 95) :: Init_int8 (Int.repr 99) ::
+                Init_int8 (Int.repr 108) :: Init_int8 (Int.repr 105) ::
+                Init_int8 (Int.repr 101) :: Init_int8 (Int.repr 110) ::
+                Init_int8 (Int.repr 116) :: Init_int8 (Int.repr 46) ::
+                Init_int8 (Int.repr 99) :: Init_int8 (Int.repr 0) :: nil);
+  gvar_readonly := true;
+  gvar_volatile := false
+|}.
+
+Definition v___stringlit_29 := {|
+  gvar_info := (tarray tschar 3);
+  gvar_init := (Init_int8 (Int.repr 73) :: Init_int8 (Int.repr 68) ::
+                Init_int8 (Int.repr 0) :: nil);
+  gvar_readonly := true;
+  gvar_volatile := false
+|}.
+
+Definition v___stringlit_26 := {|
+  gvar_info := (tarray tschar 4);
+  gvar_init := (Init_int8 (Int.repr 66) :: Init_int8 (Int.repr 111) ::
+                Init_int8 (Int.repr 98) :: Init_int8 (Int.repr 0) :: nil);
   gvar_readonly := true;
   gvar_volatile := false
 |}.
@@ -397,6 +498,16 @@ Definition v___stringlit_8 := {|
   gvar_volatile := false
 |}.
 
+Definition v___stringlit_25 := {|
+  gvar_info := (tarray tschar 7);
+  gvar_init := (Init_int8 (Int.repr 67) :: Init_int8 (Int.repr 108) ::
+                Init_int8 (Int.repr 97) :: Init_int8 (Int.repr 105) ::
+                Init_int8 (Int.repr 114) :: Init_int8 (Int.repr 101) ::
+                Init_int8 (Int.repr 0) :: nil);
+  gvar_readonly := true;
+  gvar_volatile := false
+|}.
+
 Definition v___stringlit_16 := {|
   gvar_info := (tarray tschar 6);
   gvar_init := (Init_int8 (Int.repr 76) :: Init_int8 (Int.repr 65) ::
@@ -442,6 +553,15 @@ Definition v___stringlit_3 := {|
   gvar_volatile := false
 |}.
 
+Definition v___stringlit_27 := {|
+  gvar_info := (tarray tschar 6);
+  gvar_init := (Init_int8 (Int.repr 65) :: Init_int8 (Int.repr 108) ::
+                Init_int8 (Int.repr 105) :: Init_int8 (Int.repr 99) ::
+                Init_int8 (Int.repr 101) :: Init_int8 (Int.repr 0) :: nil);
+  gvar_readonly := true;
+  gvar_volatile := false
+|}.
+
 Definition v___stringlit_1 := {|
   gvar_info := (tarray tschar 17);
   gvar_init := (Init_int8 (Int.repr 114) :: Init_int8 (Int.repr 101) ::
@@ -470,6 +590,15 @@ Definition v___stringlit_6 := {|
                 Init_int8 (Int.repr 61) :: Init_int8 (Int.repr 84) ::
                 Init_int8 (Int.repr 114) :: Init_int8 (Int.repr 117) ::
                 Init_int8 (Int.repr 101) :: Init_int8 (Int.repr 0) :: nil);
+  gvar_readonly := true;
+  gvar_volatile := false
+|}.
+
+Definition v___stringlit_24 := {|
+  gvar_info := (tarray tschar 5);
+  gvar_init := (Init_int8 (Int.repr 68) :: Init_int8 (Int.repr 101) ::
+                Init_int8 (Int.repr 97) :: Init_int8 (Int.repr 110) ::
+                Init_int8 (Int.repr 0) :: nil);
   gvar_readonly := true;
   gvar_volatile := false
 |}.
@@ -504,25 +633,20 @@ Definition v___stringlit_22 := {|
   gvar_volatile := false
 |}.
 
-Definition v___stringlit_2 := {|
-  gvar_info := (tarray tschar 15);
-  gvar_init := (Init_int8 (Int.repr 114) :: Init_int8 (Int.repr 101) ::
-                Init_int8 (Int.repr 108) :: Init_int8 (Int.repr 97) ::
-                Init_int8 (Int.repr 116) :: Init_int8 (Int.repr 105) ::
-                Init_int8 (Int.repr 111) :: Init_int8 (Int.repr 110) ::
-                Init_int8 (Int.repr 95) :: Init_int8 (Int.repr 109) ::
-                Init_int8 (Int.repr 101) :: Init_int8 (Int.repr 109) ::
-                Init_int8 (Int.repr 46) :: Init_int8 (Int.repr 99) ::
-                Init_int8 (Int.repr 0) :: nil);
-  gvar_readonly := true;
-  gvar_volatile := false
-|}.
-
 Definition v___stringlit_7 := {|
   gvar_info := (tarray tschar 7);
   gvar_init := (Init_int8 (Int.repr 99) :: Init_int8 (Int.repr 117) ::
                 Init_int8 (Int.repr 114) :: Init_int8 (Int.repr 115) ::
                 Init_int8 (Int.repr 111) :: Init_int8 (Int.repr 114) ::
+                Init_int8 (Int.repr 0) :: nil);
+  gvar_readonly := true;
+  gvar_volatile := false
+|}.
+
+Definition v___stringlit_28 := {|
+  gvar_info := (tarray tschar 5);
+  gvar_init := (Init_int8 (Int.repr 78) :: Init_int8 (Int.repr 97) ::
+                Init_int8 (Int.repr 109) :: Init_int8 (Int.repr 101) ::
                 Init_int8 (Int.repr 0) :: nil);
   gvar_readonly := true;
   gvar_volatile := false
@@ -562,6 +686,21 @@ Definition v___stringlit_20 := {|
                 Init_int8 (Int.repr 58) :: Init_int8 (Int.repr 32) ::
                 Init_int8 (Int.repr 37) :: Init_int8 (Int.repr 100) ::
                 Init_int8 (Int.repr 41) :: Init_int8 (Int.repr 32) ::
+                Init_int8 (Int.repr 0) :: nil);
+  gvar_readonly := true;
+  gvar_volatile := false
+|}.
+
+Definition v___stringlit_2 := {|
+  gvar_info := (tarray tschar 17);
+  gvar_init := (Init_int8 (Int.repr 46) :: Init_int8 (Int.repr 47) ::
+                Init_int8 (Int.repr 114) :: Init_int8 (Int.repr 101) ::
+                Init_int8 (Int.repr 108) :: Init_int8 (Int.repr 97) ::
+                Init_int8 (Int.repr 116) :: Init_int8 (Int.repr 105) ::
+                Init_int8 (Int.repr 111) :: Init_int8 (Int.repr 110) ::
+                Init_int8 (Int.repr 95) :: Init_int8 (Int.repr 109) ::
+                Init_int8 (Int.repr 101) :: Init_int8 (Int.repr 109) ::
+                Init_int8 (Int.repr 46) :: Init_int8 (Int.repr 99) ::
                 Init_int8 (Int.repr 0) :: nil);
   gvar_readonly := true;
   gvar_volatile := false
@@ -825,7 +964,7 @@ Definition f_RL_DeleteRelation := {|
         (Evar _printf (Tfunction (Tcons (tptr tschar) Tnil) tint
                         {|cc_vararg:=true; cc_unproto:=false; cc_structret:=false|}))
         ((Evar ___stringlit_3 (tarray tschar 30)) ::
-         (Evar ___stringlit_2 (tarray tschar 15)) ::
+         (Evar ___stringlit_2 (tarray tschar 17)) ::
          (Econst_int (Int.repr 202) tint) ::
          (Evar ___stringlit_1 (tarray tschar 17)) :: nil))
       (Scall None (Evar _abort (Tfunction Tnil tvoid cc_default)) nil)))
@@ -866,7 +1005,7 @@ Definition f_RL_NewCursor := {|
         (Evar _printf (Tfunction (Tcons (tptr tschar) Tnil) tint
                         {|cc_vararg:=true; cc_unproto:=false; cc_structret:=false|}))
         ((Evar ___stringlit_3 (tarray tschar 30)) ::
-         (Evar ___stringlit_2 (tarray tschar 15)) ::
+         (Evar ___stringlit_2 (tarray tschar 17)) ::
          (Econst_int (Int.repr 210) tint) ::
          (Evar ___stringlit_1 (tarray tschar 17)) :: nil))
       (Scall None (Evar _abort (Tfunction Tnil tvoid cc_default)) nil)))
@@ -946,7 +1085,7 @@ Definition f_RL_CursorIsValid := {|
         (Evar _printf (Tfunction (Tcons (tptr tschar) Tnil) tint
                         {|cc_vararg:=true; cc_unproto:=false; cc_structret:=false|}))
         ((Evar ___stringlit_3 (tarray tschar 30)) ::
-         (Evar ___stringlit_2 (tarray tschar 15)) ::
+         (Evar ___stringlit_2 (tarray tschar 17)) ::
          (Econst_int (Int.repr 229) tint) ::
          (Evar ___stringlit_4 (tarray tschar 15)) :: nil))
       (Scall None (Evar _abort (Tfunction Tnil tvoid cc_default)) nil)))
@@ -975,7 +1114,7 @@ Definition f_RL_PutRecord := {|
         (Evar _printf (Tfunction (Tcons (tptr tschar) Tnil) tint
                         {|cc_vararg:=true; cc_unproto:=false; cc_structret:=false|}))
         ((Evar ___stringlit_3 (tarray tschar 30)) ::
-         (Evar ___stringlit_2 (tarray tschar 15)) ::
+         (Evar ___stringlit_2 (tarray tschar 17)) ::
          (Econst_int (Int.repr 235) tint) ::
          (Evar ___stringlit_4 (tarray tschar 15)) :: nil))
       (Scall None (Evar _abort (Tfunction Tnil tvoid cc_default)) nil)))
@@ -1221,7 +1360,7 @@ Definition f_RL_GetRecord := {|
           (Evar _printf (Tfunction (Tcons (tptr tschar) Tnil) tint
                           {|cc_vararg:=true; cc_unproto:=false; cc_structret:=false|}))
           ((Evar ___stringlit_3 (tarray tschar 30)) ::
-           (Evar ___stringlit_2 (tarray tschar 15)) ::
+           (Evar ___stringlit_2 (tarray tschar 17)) ::
            (Econst_int (Int.repr 295) tint) ::
            (Evar ___stringlit_5 (tarray tschar 24)) :: nil))
         (Scall None (Evar _abort (Tfunction Tnil tvoid cc_default)) nil))))
@@ -1302,7 +1441,7 @@ Definition f_RL_GetKey := {|
           (Evar _printf (Tfunction (Tcons (tptr tschar) Tnil) tint
                           {|cc_vararg:=true; cc_unproto:=false; cc_structret:=false|}))
           ((Evar ___stringlit_3 (tarray tschar 30)) ::
-           (Evar ___stringlit_2 (tarray tschar 15)) ::
+           (Evar ___stringlit_2 (tarray tschar 17)) ::
            (Econst_int (Int.repr 306) tint) ::
            (Evar ___stringlit_6 (tarray tschar 22)) :: nil))
         (Scall None (Evar _abort (Tfunction Tnil tvoid cc_default)) nil))))
@@ -1376,7 +1515,7 @@ Definition f_goToKey := {|
         (Evar _printf (Tfunction (Tcons (tptr tschar) Tnil) tint
                         {|cc_vararg:=true; cc_unproto:=false; cc_structret:=false|}))
         ((Evar ___stringlit_3 (tarray tschar 30)) ::
-         (Evar ___stringlit_2 (tarray tschar 15)) ::
+         (Evar ___stringlit_2 (tarray tschar 17)) ::
          (Econst_int (Int.repr 317) tint) ::
          (Evar ___stringlit_4 (tarray tschar 15)) :: nil))
       (Scall None (Evar _abort (Tfunction Tnil tvoid cc_default)) nil)))
@@ -1476,7 +1615,7 @@ Definition f_RL_MoveToFirst := {|
         (Evar _printf (Tfunction (Tcons (tptr tschar) Tnil) tint
                         {|cc_vararg:=true; cc_unproto:=false; cc_structret:=false|}))
         ((Evar ___stringlit_3 (tarray tschar 30)) ::
-         (Evar ___stringlit_2 (tarray tschar 15)) ::
+         (Evar ___stringlit_2 (tarray tschar 17)) ::
          (Econst_int (Int.repr 357) tint) ::
          (Evar ___stringlit_7 (tarray tschar 7)) :: nil))
       (Scall None (Evar _abort (Tfunction Tnil tvoid cc_default)) nil)))
@@ -2049,7 +2188,7 @@ Definition f_RL_IsEmpty := {|
         (Evar _printf (Tfunction (Tcons (tptr tschar) Tnil) tint
                         {|cc_vararg:=true; cc_unproto:=false; cc_structret:=false|}))
         ((Evar ___stringlit_3 (tarray tschar 30)) ::
-         (Evar ___stringlit_2 (tarray tschar 15)) ::
+         (Evar ___stringlit_2 (tarray tschar 17)) ::
          (Econst_int (Int.repr 459) tint) ::
          (Evar ___stringlit_4 (tarray tschar 15)) :: nil))
       (Scall None (Evar _abort (Tfunction Tnil tvoid cc_default)) nil)))
@@ -2095,7 +2234,7 @@ Definition f_RL_NumRecords := {|
         (Evar _printf (Tfunction (Tcons (tptr tschar) Tnil) tint
                         {|cc_vararg:=true; cc_unproto:=false; cc_structret:=false|}))
         ((Evar ___stringlit_3 (tarray tschar 30)) ::
-         (Evar ___stringlit_2 (tarray tschar 15)) ::
+         (Evar ___stringlit_2 (tarray tschar 17)) ::
          (Econst_int (Int.repr 468) tint) ::
          (Evar ___stringlit_4 (tarray tschar 15)) :: nil))
       (Scall None (Evar _abort (Tfunction Tnil tvoid cc_default)) nil)))
@@ -2132,7 +2271,7 @@ Definition f_RL_PrintTree := {|
         (Evar _printf (Tfunction (Tcons (tptr tschar) Tnil) tint
                         {|cc_vararg:=true; cc_unproto:=false; cc_structret:=false|}))
         ((Evar ___stringlit_3 (tarray tschar 30)) ::
-         (Evar ___stringlit_2 (tarray tschar 15)) ::
+         (Evar ___stringlit_2 (tarray tschar 17)) ::
          (Econst_int (Int.repr 476) tint) ::
          (Evar ___stringlit_1 (tarray tschar 17)) :: nil))
       (Scall None (Evar _abort (Tfunction Tnil tvoid cc_default)) nil)))
@@ -2153,7 +2292,7 @@ Definition f_RL_PrintTree := {|
             (Evar _printf (Tfunction (Tcons (tptr tschar) Tnil) tint
                             {|cc_vararg:=true; cc_unproto:=false; cc_structret:=false|}))
             ((Evar ___stringlit_3 (tarray tschar 30)) ::
-             (Evar ___stringlit_2 (tarray tschar 15)) ::
+             (Evar ___stringlit_2 (tarray tschar 17)) ::
              (Econst_int (Int.repr 477) tint) ::
              (Evar ___stringlit_8 (tarray tschar 23)) :: nil))
           (Scall None (Evar _abort (Tfunction Tnil tvoid cc_default)) nil))))
@@ -2187,7 +2326,7 @@ Definition f_RL_PrintCursor := {|
         (Evar _printf (Tfunction (Tcons (tptr tschar) Tnil) tint
                         {|cc_vararg:=true; cc_unproto:=false; cc_structret:=false|}))
         ((Evar ___stringlit_3 (tarray tschar 30)) ::
-         (Evar ___stringlit_2 (tarray tschar 15)) ::
+         (Evar ___stringlit_2 (tarray tschar 17)) ::
          (Econst_int (Int.repr 485) tint) ::
          (Evar ___stringlit_4 (tarray tschar 15)) :: nil))
       (Scall None (Evar _abort (Tfunction Tnil tvoid cc_default)) nil)))
@@ -2258,7 +2397,7 @@ Definition f_splitnode := {|
   fn_return := tvoid;
   fn_callconv := cc_default;
   fn_params := ((_node, (tptr (Tstruct _BtNode noattr))) ::
-                (_entry, (tptr (Tstruct _Entry noattr))) ::
+                (_entry__2, (tptr (Tstruct _Entry noattr))) ::
                 (_isLeaf, tint) :: nil);
   fn_vars := ((_allEntries, (tarray (Tstruct _Entry noattr) 16)) :: nil);
   fn_temps := ((_newNode, (tptr (Tstruct _BtNode noattr))) :: (_i, tint) ::
@@ -2283,7 +2422,7 @@ Definition f_splitnode := {|
     (Ssequence
       (Sset _t'29
         (Efield
-          (Ederef (Etempvar _entry (tptr (Tstruct _Entry noattr)))
+          (Ederef (Etempvar _entry__2 (tptr (Tstruct _Entry noattr)))
             (Tstruct _Entry noattr)) _key tulong))
       (Scall (Some _t'1)
         (Evar _findRecordIndex (Tfunction
@@ -2314,7 +2453,7 @@ Definition f_splitnode := {|
             (Evar _printf (Tfunction (Tcons (tptr tschar) Tnil) tint
                             {|cc_vararg:=true; cc_unproto:=false; cc_structret:=false|}))
             ((Evar ___stringlit_3 (tarray tschar 30)) ::
-             (Evar ___stringlit_2 (tarray tschar 15)) ::
+             (Evar ___stringlit_2 (tarray tschar 17)) ::
              (Econst_int (Int.repr 524) tint) ::
              (Evar ___stringlit_9 (tarray tschar 8)) :: nil))
           (Scall None (Evar _abort (Tfunction Tnil tvoid cc_default)) nil)))
@@ -2398,7 +2537,7 @@ Definition f_splitnode := {|
                   (Sset _t'25
                     (Efield
                       (Ederef
-                        (Etempvar _entry (tptr (Tstruct _Entry noattr)))
+                        (Etempvar _entry__2 (tptr (Tstruct _Entry noattr)))
                         (Tstruct _Entry noattr)) _key tulong))
                   (Sassign
                     (Efield
@@ -2415,7 +2554,7 @@ Definition f_splitnode := {|
                       (Efield
                         (Efield
                           (Ederef
-                            (Etempvar _entry (tptr (Tstruct _Entry noattr)))
+                            (Etempvar _entry__2 (tptr (Tstruct _Entry noattr)))
                             (Tstruct _Entry noattr)) _ptr
                           (Tunion _Child_or_Record noattr)) _record
                         (tptr tvoid)))
@@ -2671,7 +2810,7 @@ Definition f_splitnode := {|
                                 (Sassign
                                   (Efield
                                     (Ederef
-                                      (Etempvar _entry (tptr (Tstruct _Entry noattr)))
+                                      (Etempvar _entry__2 (tptr (Tstruct _Entry noattr)))
                                       (Tstruct _Entry noattr)) _key tulong)
                                   (Etempvar _t'17 tulong)))
                               (Ssequence
@@ -2679,7 +2818,7 @@ Definition f_splitnode := {|
                                   (Efield
                                     (Efield
                                       (Ederef
-                                        (Etempvar _entry (tptr (Tstruct _Entry noattr)))
+                                        (Etempvar _entry__2 (tptr (Tstruct _Entry noattr)))
                                         (Tstruct _Entry noattr)) _ptr
                                       (Tunion _Child_or_Record noattr))
                                     _child (tptr (Tstruct _BtNode noattr)))
@@ -2753,7 +2892,7 @@ Definition f_splitnode := {|
                   (Sset _t'14
                     (Efield
                       (Ederef
-                        (Etempvar _entry (tptr (Tstruct _Entry noattr)))
+                        (Etempvar _entry__2 (tptr (Tstruct _Entry noattr)))
                         (Tstruct _Entry noattr)) _key tulong))
                   (Sassign
                     (Efield
@@ -2770,7 +2909,7 @@ Definition f_splitnode := {|
                       (Efield
                         (Efield
                           (Ederef
-                            (Etempvar _entry (tptr (Tstruct _Entry noattr)))
+                            (Etempvar _entry__2 (tptr (Tstruct _Entry noattr)))
                             (Tstruct _Entry noattr)) _ptr
                           (Tunion _Child_or_Record noattr)) _child
                         (tptr (Tstruct _BtNode noattr))))
@@ -3055,7 +3194,7 @@ Definition f_splitnode := {|
                                   (Sassign
                                     (Efield
                                       (Ederef
-                                        (Etempvar _entry (tptr (Tstruct _Entry noattr)))
+                                        (Etempvar _entry__2 (tptr (Tstruct _Entry noattr)))
                                         (Tstruct _Entry noattr)) _key tulong)
                                     (Etempvar _t'5 tulong)))
                                 (Ssequence
@@ -3063,7 +3202,7 @@ Definition f_splitnode := {|
                                     (Efield
                                       (Efield
                                         (Ederef
-                                          (Etempvar _entry (tptr (Tstruct _Entry noattr)))
+                                          (Etempvar _entry__2 (tptr (Tstruct _Entry noattr)))
                                           (Tstruct _Entry noattr)) _ptr
                                         (Tunion _Child_or_Record noattr))
                                       _child (tptr (Tstruct _BtNode noattr)))
@@ -3157,7 +3296,7 @@ Definition f_putEntry := {|
                 (Evar _printf (Tfunction (Tcons (tptr tschar) Tnil) tint
                                 {|cc_vararg:=true; cc_unproto:=false; cc_structret:=false|}))
                 ((Evar ___stringlit_3 (tarray tschar 30)) ::
-                 (Evar ___stringlit_2 (tarray tschar 15)) ::
+                 (Evar ___stringlit_2 (tarray tschar 17)) ::
                  (Econst_int (Int.repr 686) tint) ::
                  (Evar ___stringlit_10 (tarray tschar 9)) :: nil))
               (Scall None (Evar _abort (Tfunction Tnil tvoid cc_default))
@@ -4165,7 +4304,7 @@ Definition f_findChildIndex := {|
             (Evar _printf (Tfunction (Tcons (tptr tschar) Tnil) tint
                             {|cc_vararg:=true; cc_unproto:=false; cc_structret:=false|}))
             ((Evar ___stringlit_3 (tarray tschar 30)) ::
-             (Evar ___stringlit_2 (tarray tschar 15)) ::
+             (Evar ___stringlit_2 (tarray tschar 17)) ::
              (Econst_int (Int.repr 1152) tint) ::
              (Evar ___stringlit_11 (tarray tschar 18)) :: nil))
           (Scall None (Evar _abort (Tfunction Tnil tvoid cc_default)) nil))))
@@ -4237,7 +4376,7 @@ Definition f_findRecordIndex := {|
             (Evar _printf (Tfunction (Tcons (tptr tschar) Tnil) tint
                             {|cc_vararg:=true; cc_unproto:=false; cc_structret:=false|}))
             ((Evar ___stringlit_3 (tarray tschar 30)) ::
-             (Evar ___stringlit_2 (tarray tschar 15)) ::
+             (Evar ___stringlit_2 (tarray tschar 17)) ::
              (Econst_int (Int.repr 1168) tint) ::
              (Evar ___stringlit_12 (tarray tschar 19)) :: nil))
           (Scall None (Evar _abort (Tfunction Tnil tvoid cc_default)) nil))))
@@ -4424,7 +4563,7 @@ Definition f_moveToFirst := {|
         (Evar _printf (Tfunction (Tcons (tptr tschar) Tnil) tint
                         {|cc_vararg:=true; cc_unproto:=false; cc_structret:=false|}))
         ((Evar ___stringlit_3 (tarray tschar 30)) ::
-         (Evar ___stringlit_2 (tarray tschar 15)) ::
+         (Evar ___stringlit_2 (tarray tschar 17)) ::
          (Econst_int (Int.repr 1217) tint) ::
          (Evar ___stringlit_13 (tarray tschar 13)) :: nil))
       (Scall None (Evar _abort (Tfunction Tnil tvoid cc_default)) nil)))
@@ -4438,7 +4577,7 @@ Definition f_moveToFirst := {|
           (Evar _printf (Tfunction (Tcons (tptr tschar) Tnil) tint
                           {|cc_vararg:=true; cc_unproto:=false; cc_structret:=false|}))
           ((Evar ___stringlit_3 (tarray tschar 30)) ::
-           (Evar ___stringlit_2 (tarray tschar 15)) ::
+           (Evar ___stringlit_2 (tarray tschar 17)) ::
            (Econst_int (Int.repr 1218) tint) ::
            (Evar ___stringlit_4 (tarray tschar 15)) :: nil))
         (Scall None (Evar _abort (Tfunction Tnil tvoid cc_default)) nil)))
@@ -4451,7 +4590,7 @@ Definition f_moveToFirst := {|
             (Evar _printf (Tfunction (Tcons (tptr tschar) Tnil) tint
                             {|cc_vararg:=true; cc_unproto:=false; cc_structret:=false|}))
             ((Evar ___stringlit_3 (tarray tschar 30)) ::
-             (Evar ___stringlit_2 (tarray tschar 15)) ::
+             (Evar ___stringlit_2 (tarray tschar 17)) ::
              (Econst_int (Int.repr 1219) tint) ::
              (Evar ___stringlit_14 (tarray tschar 11)) :: nil))
           (Scall None (Evar _abort (Tfunction Tnil tvoid cc_default)) nil)))
@@ -4541,7 +4680,7 @@ Definition f_moveToLast := {|
         (Evar _printf (Tfunction (Tcons (tptr tschar) Tnil) tint
                         {|cc_vararg:=true; cc_unproto:=false; cc_structret:=false|}))
         ((Evar ___stringlit_3 (tarray tschar 30)) ::
-         (Evar ___stringlit_2 (tarray tschar 15)) ::
+         (Evar ___stringlit_2 (tarray tschar 17)) ::
          (Econst_int (Int.repr 1236) tint) ::
          (Evar ___stringlit_13 (tarray tschar 13)) :: nil))
       (Scall None (Evar _abort (Tfunction Tnil tvoid cc_default)) nil)))
@@ -4555,7 +4694,7 @@ Definition f_moveToLast := {|
           (Evar _printf (Tfunction (Tcons (tptr tschar) Tnil) tint
                           {|cc_vararg:=true; cc_unproto:=false; cc_structret:=false|}))
           ((Evar ___stringlit_3 (tarray tschar 30)) ::
-           (Evar ___stringlit_2 (tarray tschar 15)) ::
+           (Evar ___stringlit_2 (tarray tschar 17)) ::
            (Econst_int (Int.repr 1237) tint) ::
            (Evar ___stringlit_4 (tarray tschar 15)) :: nil))
         (Scall None (Evar _abort (Tfunction Tnil tvoid cc_default)) nil)))
@@ -4568,7 +4707,7 @@ Definition f_moveToLast := {|
             (Evar _printf (Tfunction (Tcons (tptr tschar) Tnil) tint
                             {|cc_vararg:=true; cc_unproto:=false; cc_structret:=false|}))
             ((Evar ___stringlit_3 (tarray tschar 30)) ::
-             (Evar ___stringlit_2 (tarray tschar 15)) ::
+             (Evar ___stringlit_2 (tarray tschar 17)) ::
              (Econst_int (Int.repr 1238) tint) ::
              (Evar ___stringlit_14 (tarray tschar 11)) :: nil))
           (Scall None (Evar _abort (Tfunction Tnil tvoid cc_default)) nil)))
@@ -4980,6 +5119,764 @@ Definition f_printCursor := {|
       ((Evar ___stringlit_19 (tarray tschar 2)) :: nil))))
 |}.
 
+Definition f_btree_create_index := {|
+  fn_return := (tptr (Tstruct _db_cursor_t noattr));
+  fn_callconv := cc_default;
+  fn_params := nil;
+  fn_vars := nil;
+  fn_temps := ((_t'1, (tptr (Tstruct _Relation noattr))) :: nil);
+  fn_body :=
+(Ssequence
+  (Scall (Some _t'1)
+    (Evar _RL_NewRelation (Tfunction Tnil (tptr (Tstruct _Relation noattr))
+                            cc_default)) nil)
+  (Sreturn (Some (Ecast (Etempvar _t'1 (tptr (Tstruct _Relation noattr)))
+                   (tptr (Tstruct _db_cursor_t noattr))))))
+|}.
+
+Definition f_btree_create_cursor := {|
+  fn_return := (tptr (Tstruct _db_cursor_t noattr));
+  fn_callconv := cc_default;
+  fn_params := ((_env, (tptr (Tstruct _index_t noattr))) :: nil);
+  fn_vars := nil;
+  fn_temps := ((_tree, (tptr (Tstruct _Relation noattr))) ::
+               (_cursor, (tptr (Tstruct _BtreeCursor noattr))) ::
+               (_t'3, (tptr (Tstruct _Cursor noattr))) :: (_t'2, tint) ::
+               (_t'1, (tptr tvoid)) :: nil);
+  fn_body :=
+(Ssequence
+  (Sset _tree
+    (Ecast (Etempvar _env (tptr (Tstruct _index_t noattr)))
+      (tptr (Tstruct _Relation noattr))))
+  (Ssequence
+    (Ssequence
+      (Scall (Some _t'1)
+        (Evar _malloc (Tfunction (Tcons tulong Tnil) (tptr tvoid) cc_default))
+        ((Esizeof (Tstruct _BtreeCursor noattr) tulong) :: nil))
+      (Sset _cursor (Etempvar _t'1 (tptr tvoid))))
+    (Ssequence
+      (Sifthenelse (Ebinop One
+                     (Etempvar _cursor (tptr (Tstruct _BtreeCursor noattr)))
+                     (Ecast (Econst_int (Int.repr 0) tint) (tptr tvoid))
+                     tint)
+        Sskip
+        (Ssequence
+          (Scall (Some _t'2)
+            (Evar _printf (Tfunction (Tcons (tptr tschar) Tnil) tint
+                            {|cc_vararg:=true; cc_unproto:=false; cc_structret:=false|}))
+            ((Evar ___stringlit_3 (tarray tschar 30)) ::
+             (Evar ___stringlit_23 (tarray tschar 12)) ::
+             (Econst_int (Int.repr 18) tint) ::
+             (Evar ___stringlit_4 (tarray tschar 15)) :: nil))
+          (Scall None (Evar _abort (Tfunction Tnil tvoid cc_default)) nil)))
+      (Ssequence
+        (Sassign
+          (Efield
+            (Ederef (Etempvar _cursor (tptr (Tstruct _BtreeCursor noattr)))
+              (Tstruct _BtreeCursor noattr)) _btree
+            (tptr (Tstruct _Relation noattr)))
+          (Etempvar _tree (tptr (Tstruct _Relation noattr))))
+        (Ssequence
+          (Ssequence
+            (Scall (Some _t'3)
+              (Evar _RL_NewCursor (Tfunction
+                                    (Tcons (tptr (Tstruct _Relation noattr))
+                                      Tnil) (tptr (Tstruct _Cursor noattr))
+                                    cc_default))
+              ((Etempvar _tree (tptr (Tstruct _Relation noattr))) :: nil))
+            (Sassign
+              (Efield
+                (Ederef
+                  (Etempvar _cursor (tptr (Tstruct _BtreeCursor noattr)))
+                  (Tstruct _BtreeCursor noattr)) _cur
+                (tptr (Tstruct _Cursor noattr)))
+              (Etempvar _t'3 (tptr (Tstruct _Cursor noattr)))))
+          (Sreturn (Some (Ecast
+                           (Etempvar _cursor (tptr (Tstruct _BtreeCursor noattr)))
+                           (tptr (Tstruct _db_cursor_t noattr))))))))))
+|}.
+
+Definition f_btree_cardinality := {|
+  fn_return := tulong;
+  fn_callconv := cc_default;
+  fn_params := ((_env, (tptr (Tstruct _db_cursor_t noattr))) :: nil);
+  fn_vars := nil;
+  fn_temps := ((_cursor, (tptr (Tstruct _BtreeCursor noattr))) ::
+               (_t'1, tulong) :: (_t'2, (tptr (Tstruct _Cursor noattr))) ::
+               nil);
+  fn_body :=
+(Ssequence
+  (Sset _cursor
+    (Ecast (Etempvar _env (tptr (Tstruct _db_cursor_t noattr)))
+      (tptr (Tstruct _BtreeCursor noattr))))
+  (Ssequence
+    (Ssequence
+      (Sset _t'2
+        (Efield
+          (Ederef (Etempvar _cursor (tptr (Tstruct _BtreeCursor noattr)))
+            (Tstruct _BtreeCursor noattr)) _cur
+          (tptr (Tstruct _Cursor noattr))))
+      (Scall (Some _t'1)
+        (Evar _RL_NumRecords (Tfunction
+                               (Tcons (tptr (Tstruct _Cursor noattr)) Tnil)
+                               tulong cc_default))
+        ((Etempvar _t'2 (tptr (Tstruct _Cursor noattr))) :: nil)))
+    (Sreturn (Some (Etempvar _t'1 tulong)))))
+|}.
+
+Definition f_btree_move_to_next := {|
+  fn_return := tint;
+  fn_callconv := cc_default;
+  fn_params := ((_env, (tptr (Tstruct _db_cursor_t noattr))) :: nil);
+  fn_vars := nil;
+  fn_temps := ((_cursor, (tptr (Tstruct _BtreeCursor noattr))) ::
+               (_t'1, tint) :: (_t'2, (tptr (Tstruct _Cursor noattr))) ::
+               nil);
+  fn_body :=
+(Ssequence
+  (Sset _cursor
+    (Ecast (Etempvar _env (tptr (Tstruct _db_cursor_t noattr)))
+      (tptr (Tstruct _BtreeCursor noattr))))
+  (Ssequence
+    (Ssequence
+      (Sset _t'2
+        (Efield
+          (Ederef (Etempvar _cursor (tptr (Tstruct _BtreeCursor noattr)))
+            (Tstruct _BtreeCursor noattr)) _cur
+          (tptr (Tstruct _Cursor noattr))))
+      (Scall (Some _t'1)
+        (Evar _RL_MoveToNextValid (Tfunction
+                                    (Tcons (tptr (Tstruct _Cursor noattr))
+                                      Tnil) tint cc_default))
+        ((Etempvar _t'2 (tptr (Tstruct _Cursor noattr))) :: nil)))
+    (Sreturn (Some (Etempvar _t'1 tint)))))
+|}.
+
+Definition f_btree_move_to_first := {|
+  fn_return := tint;
+  fn_callconv := cc_default;
+  fn_params := ((_env, (tptr (Tstruct _db_cursor_t noattr))) :: nil);
+  fn_vars := nil;
+  fn_temps := ((_cursor, (tptr (Tstruct _BtreeCursor noattr))) ::
+               (_t'1, tint) :: (_t'2, (tptr (Tstruct _Cursor noattr))) ::
+               nil);
+  fn_body :=
+(Ssequence
+  (Sset _cursor
+    (Ecast (Etempvar _env (tptr (Tstruct _db_cursor_t noattr)))
+      (tptr (Tstruct _BtreeCursor noattr))))
+  (Ssequence
+    (Ssequence
+      (Sset _t'2
+        (Efield
+          (Ederef (Etempvar _cursor (tptr (Tstruct _BtreeCursor noattr)))
+            (Tstruct _BtreeCursor noattr)) _cur
+          (tptr (Tstruct _Cursor noattr))))
+      (Scall (Some _t'1)
+        (Evar _RL_MoveToFirst (Tfunction
+                                (Tcons (tptr (Tstruct _Cursor noattr)) Tnil)
+                                tint cc_default))
+        ((Etempvar _t'2 (tptr (Tstruct _Cursor noattr))) :: nil)))
+    (Sreturn (Some (Etempvar _t'1 tint)))))
+|}.
+
+Definition f_btree_go_to_key := {|
+  fn_return := tint;
+  fn_callconv := cc_default;
+  fn_params := ((_env, (tptr (Tstruct _db_cursor_t noattr))) ::
+                (_key, (tptr (Tstruct _key_t noattr))) :: nil);
+  fn_vars := nil;
+  fn_temps := ((_cursor, (tptr (Tstruct _BtreeCursor noattr))) ::
+               (_k, (tptr (Tunion _entry noattr))) :: (_t'1, tint) ::
+               (_t'4, tulong) :: (_t'3, (tptr (Tstruct _Cursor noattr))) ::
+               (_t'2, (tptr (Tstruct _Cursor noattr))) :: nil);
+  fn_body :=
+(Ssequence
+  (Sset _cursor
+    (Ecast (Etempvar _env (tptr (Tstruct _db_cursor_t noattr)))
+      (tptr (Tstruct _BtreeCursor noattr))))
+  (Ssequence
+    (Sset _k
+      (Ecast (Etempvar _key (tptr (Tstruct _key_t noattr)))
+        (tptr (Tunion _entry noattr))))
+    (Ssequence
+      (Ssequence
+        (Sset _t'3
+          (Efield
+            (Ederef (Etempvar _cursor (tptr (Tstruct _BtreeCursor noattr)))
+              (Tstruct _BtreeCursor noattr)) _cur
+            (tptr (Tstruct _Cursor noattr))))
+        (Ssequence
+          (Sset _t'4
+            (Efield
+              (Ederef (Etempvar _k (tptr (Tunion _entry noattr)))
+                (Tunion _entry noattr)) _int_cont tulong))
+          (Scall None
+            (Evar _goToKey (Tfunction
+                             (Tcons (tptr (Tstruct _Cursor noattr))
+                               (Tcons tulong Tnil)) tvoid cc_default))
+            ((Etempvar _t'3 (tptr (Tstruct _Cursor noattr))) ::
+             (Etempvar _t'4 tulong) :: nil))))
+      (Ssequence
+        (Ssequence
+          (Sset _t'2
+            (Efield
+              (Ederef (Etempvar _cursor (tptr (Tstruct _BtreeCursor noattr)))
+                (Tstruct _BtreeCursor noattr)) _cur
+              (tptr (Tstruct _Cursor noattr))))
+          (Scall (Some _t'1)
+            (Evar _RL_CursorIsValid (Tfunction
+                                      (Tcons (tptr (Tstruct _Cursor noattr))
+                                        Tnil) tint cc_default))
+            ((Etempvar _t'2 (tptr (Tstruct _Cursor noattr))) :: nil)))
+        (Sreturn (Some (Etempvar _t'1 tint)))))))
+|}.
+
+Definition f_btree_cursor_has_next := {|
+  fn_return := tint;
+  fn_callconv := cc_default;
+  fn_params := ((_env, (tptr (Tstruct _db_cursor_t noattr))) :: nil);
+  fn_vars := nil;
+  fn_temps := ((_cursor, (tptr (Tstruct _BtreeCursor noattr))) ::
+               (_t'1, tint) :: (_t'2, (tptr (Tstruct _Cursor noattr))) ::
+               nil);
+  fn_body :=
+(Ssequence
+  (Sset _cursor
+    (Ecast (Etempvar _env (tptr (Tstruct _db_cursor_t noattr)))
+      (tptr (Tstruct _BtreeCursor noattr))))
+  (Ssequence
+    (Ssequence
+      (Sset _t'2
+        (Efield
+          (Ederef (Etempvar _cursor (tptr (Tstruct _BtreeCursor noattr)))
+            (Tstruct _BtreeCursor noattr)) _cur
+          (tptr (Tstruct _Cursor noattr))))
+      (Scall (Some _t'1)
+        (Evar _RL_CursorIsValid (Tfunction
+                                  (Tcons (tptr (Tstruct _Cursor noattr))
+                                    Tnil) tint cc_default))
+        ((Etempvar _t'2 (tptr (Tstruct _Cursor noattr))) :: nil)))
+    (Sreturn (Some (Etempvar _t'1 tint)))))
+|}.
+
+Definition f_btree_put_record := {|
+  fn_return := tvoid;
+  fn_callconv := cc_default;
+  fn_params := ((_env, (tptr (Tstruct _db_cursor_t noattr))) ::
+                (_key, (tptr (Tstruct _key_t noattr))) ::
+                (_value, (tptr (Tstruct _value_t noattr))) :: nil);
+  fn_vars := nil;
+  fn_temps := ((_cursor, (tptr (Tstruct _BtreeCursor noattr))) ::
+               (_k, (tptr (Tunion _entry noattr))) :: (_t'2, tulong) ::
+               (_t'1, (tptr (Tstruct _Cursor noattr))) :: nil);
+  fn_body :=
+(Ssequence
+  (Sset _cursor
+    (Ecast (Etempvar _env (tptr (Tstruct _db_cursor_t noattr)))
+      (tptr (Tstruct _BtreeCursor noattr))))
+  (Ssequence
+    (Sset _k
+      (Ecast (Etempvar _key (tptr (Tstruct _key_t noattr)))
+        (tptr (Tunion _entry noattr))))
+    (Ssequence
+      (Sset _t'1
+        (Efield
+          (Ederef (Etempvar _cursor (tptr (Tstruct _BtreeCursor noattr)))
+            (Tstruct _BtreeCursor noattr)) _cur
+          (tptr (Tstruct _Cursor noattr))))
+      (Ssequence
+        (Sset _t'2
+          (Efield
+            (Ederef (Etempvar _k (tptr (Tunion _entry noattr)))
+              (Tunion _entry noattr)) _int_cont tulong))
+        (Scall None
+          (Evar _RL_PutRecord (Tfunction
+                                (Tcons (tptr (Tstruct _Cursor noattr))
+                                  (Tcons tulong (Tcons (tptr tvoid) Tnil)))
+                                tvoid cc_default))
+          ((Etempvar _t'1 (tptr (Tstruct _Cursor noattr))) ::
+           (Etempvar _t'2 tulong) ::
+           (Etempvar _value (tptr (Tstruct _value_t noattr))) :: nil))))))
+|}.
+
+Definition f_btree_get_record := {|
+  fn_return := (tptr (Tstruct _value_t noattr));
+  fn_callconv := cc_default;
+  fn_params := ((_env, (tptr (Tstruct _db_cursor_t noattr))) :: nil);
+  fn_vars := nil;
+  fn_temps := ((_cursor, (tptr (Tstruct _BtreeCursor noattr))) ::
+               (_t'1, (tptr tvoid)) ::
+               (_t'2, (tptr (Tstruct _Cursor noattr))) :: nil);
+  fn_body :=
+(Ssequence
+  (Sset _cursor
+    (Ecast (Etempvar _env (tptr (Tstruct _db_cursor_t noattr)))
+      (tptr (Tstruct _BtreeCursor noattr))))
+  (Ssequence
+    (Ssequence
+      (Sset _t'2
+        (Efield
+          (Ederef (Etempvar _cursor (tptr (Tstruct _BtreeCursor noattr)))
+            (Tstruct _BtreeCursor noattr)) _cur
+          (tptr (Tstruct _Cursor noattr))))
+      (Scall (Some _t'1)
+        (Evar _RL_GetRecord (Tfunction
+                              (Tcons (tptr (Tstruct _Cursor noattr)) Tnil)
+                              (tptr tvoid) cc_default))
+        ((Etempvar _t'2 (tptr (Tstruct _Cursor noattr))) :: nil)))
+    (Sreturn (Some (Ecast (Etempvar _t'1 (tptr tvoid))
+                     (tptr (Tstruct _value_t noattr)))))))
+|}.
+
+Definition v_btree_mtable := {|
+  gvar_info := (Tstruct _OrdIndexMtable noattr);
+  gvar_init := (Init_addrof _btree_create_index (Ptrofs.repr 0) ::
+                Init_addrof _btree_create_cursor (Ptrofs.repr 0) ::
+                Init_addrof _btree_cardinality (Ptrofs.repr 0) ::
+                Init_addrof _btree_move_to_next (Ptrofs.repr 0) ::
+                Init_addrof _btree_move_to_first (Ptrofs.repr 0) ::
+                Init_addrof _btree_go_to_key (Ptrofs.repr 0) ::
+                Init_addrof _btree_cursor_has_next (Ptrofs.repr 0) ::
+                Init_addrof _btree_put_record (Ptrofs.repr 0) ::
+                Init_addrof _btree_get_record (Ptrofs.repr 0) :: nil);
+  gvar_readonly := false;
+  gvar_volatile := false
+|}.
+
+Definition f_attr_list_length := {|
+  fn_return := tulong;
+  fn_callconv := cc_default;
+  fn_params := ((_lst, (tptr (Tstruct _attribute_list noattr))) :: nil);
+  fn_vars := nil;
+  fn_temps := ((_length, tulong) :: nil);
+  fn_body :=
+(Ssequence
+  (Sset _length (Ecast (Econst_int (Int.repr 0) tint) tulong))
+  (Ssequence
+    (Swhile
+      (Ebinop One (Etempvar _lst (tptr (Tstruct _attribute_list noattr)))
+        (Ecast (Econst_int (Int.repr 0) tint) (tptr tvoid)) tint)
+      (Ssequence
+        (Sset _length
+          (Ebinop Oadd (Etempvar _length tulong)
+            (Econst_int (Int.repr 1) tint) tulong))
+        (Sset _lst
+          (Efield
+            (Ederef (Etempvar _lst (tptr (Tstruct _attribute_list noattr)))
+              (Tstruct _attribute_list noattr)) _next
+            (tptr (Tstruct _attribute_list noattr))))))
+    (Sreturn (Some (Etempvar _length tulong)))))
+|}.
+
+Definition f_index_of_pk_column := {|
+  fn_return := tint;
+  fn_callconv := cc_default;
+  fn_params := ((_lst, (tptr (Tstruct _attribute_list noattr))) ::
+                (_pk, (tptr (Tstruct _attribute_list noattr))) :: nil);
+  fn_vars := nil;
+  fn_temps := ((_ind, tint) :: (_pk_ID, (tptr tschar)) :: (_t'1, tint) ::
+               (_t'2, (tptr tschar)) :: nil);
+  fn_body :=
+(Ssequence
+  (Sset _ind (Econst_int (Int.repr 0) tint))
+  (Ssequence
+    (Sset _pk_ID
+      (Efield
+        (Ederef (Etempvar _pk (tptr (Tstruct _attribute_list noattr)))
+          (Tstruct _attribute_list noattr)) _id (tptr tschar)))
+    (Ssequence
+      (Swhile
+        (Ebinop One (Etempvar _lst (tptr (Tstruct _attribute_list noattr)))
+          (Ecast (Econst_int (Int.repr 0) tint) (tptr tvoid)) tint)
+        (Ssequence
+          (Ssequence
+            (Ssequence
+              (Sset _t'2
+                (Efield
+                  (Ederef
+                    (Etempvar _lst (tptr (Tstruct _attribute_list noattr)))
+                    (Tstruct _attribute_list noattr)) _id (tptr tschar)))
+              (Scall (Some _t'1)
+                (Evar _strcmp (Tfunction
+                                (Tcons (tptr tschar)
+                                  (Tcons (tptr tschar) Tnil)) tint
+                                cc_default))
+                ((Etempvar _pk_ID (tptr tschar)) ::
+                 (Etempvar _t'2 (tptr tschar)) :: nil)))
+            (Sifthenelse (Ebinop Oeq (Etempvar _t'1 tint)
+                           (Econst_int (Int.repr 0) tint) tint)
+              (Sreturn (Some (Etempvar _ind tint)))
+              Sskip))
+          (Ssequence
+            (Sset _ind
+              (Ebinop Oadd (Etempvar _ind tint)
+                (Econst_int (Int.repr 1) tint) tint))
+            (Sset _lst
+              (Efield
+                (Ederef
+                  (Etempvar _lst (tptr (Tstruct _attribute_list noattr)))
+                  (Tstruct _attribute_list noattr)) _next
+                (tptr (Tstruct _attribute_list noattr)))))))
+      (Sreturn (Some (Eunop Oneg (Econst_int (Int.repr 1) tint) tint))))))
+|}.
+
+Definition f_create_relation := {|
+  fn_return := (tptr (Tstruct _Cursor noattr));
+  fn_callconv := cc_default;
+  fn_params := ((_att, (tptr (Tstruct _index_attributes noattr))) :: nil);
+  fn_vars := nil;
+  fn_temps := ((_rel, (tptr (Tstruct _Relation noattr))) ::
+               (_cur, (tptr (Tstruct _Cursor noattr))) ::
+               (_t'2, (tptr (Tstruct _Cursor noattr))) ::
+               (_t'1, (tptr (Tstruct _Relation noattr))) :: (_t'4, tint) ::
+               (_t'3, (tptr (Tstruct _attribute_list noattr))) :: nil);
+  fn_body :=
+(Ssequence
+  (Ssequence
+    (Sset _t'3
+      (Efield
+        (Ederef (Etempvar _att (tptr (Tstruct _index_attributes noattr)))
+          (Tstruct _index_attributes noattr)) _pk_attrs
+        (tptr (Tstruct _attribute_list noattr))))
+    (Ssequence
+      (Sset _t'4
+        (Efield
+          (Ederef (Etempvar _t'3 (tptr (Tstruct _attribute_list noattr)))
+            (Tstruct _attribute_list noattr)) _domain tint))
+      (Sifthenelse (Ebinop One (Etempvar _t'4 tint)
+                     (Econst_int (Int.repr 0) tint) tint)
+        (Sreturn (Some (Ecast (Econst_int (Int.repr 0) tint) (tptr tvoid))))
+        Sskip)))
+  (Ssequence
+    (Ssequence
+      (Scall (Some _t'1)
+        (Evar _RL_NewRelation (Tfunction Tnil
+                                (tptr (Tstruct _Relation noattr)) cc_default))
+        nil)
+      (Sset _rel (Etempvar _t'1 (tptr (Tstruct _Relation noattr)))))
+    (Ssequence
+      (Ssequence
+        (Scall (Some _t'2)
+          (Evar _RL_NewCursor (Tfunction
+                                (Tcons (tptr (Tstruct _Relation noattr))
+                                  Tnil) (tptr (Tstruct _Cursor noattr))
+                                cc_default))
+          ((Etempvar _rel (tptr (Tstruct _Relation noattr))) :: nil))
+        (Sset _cur (Etempvar _t'2 (tptr (Tstruct _Cursor noattr)))))
+      (Sreturn (Some (Etempvar _cur (tptr (Tstruct _Cursor noattr))))))))
+|}.
+
+Definition f_fill_relation := {|
+  fn_return := (tptr (Tstruct _Relation noattr));
+  fn_callconv := cc_default;
+  fn_params := ((_arr, (tptr (Tunion _entry noattr))) ::
+                (_cur, (tptr (Tstruct _Cursor noattr))) ::
+                (_numrows, tulong) ::
+                (_att, (tptr (Tstruct _index_attributes noattr))) :: nil);
+  fn_vars := ((_key, (Tunion _entry noattr)) :: nil);
+  fn_temps := ((_numcols, tulong) :: (_pk_num, tulong) :: (_i, tulong) ::
+               (_ptr_to_row, (tptr tvoid)) :: (_t'2, tint) ::
+               (_t'1, tulong) ::
+               (_t'7, (tptr (Tstruct _attribute_list noattr))) ::
+               (_t'6, (tptr (Tstruct _attribute_list noattr))) ::
+               (_t'5, (tptr (Tstruct _attribute_list noattr))) ::
+               (_t'4, tulong) :: (_t'3, (tptr (Tstruct _Relation noattr))) ::
+               nil);
+  fn_body :=
+(Ssequence
+  (Ssequence
+    (Ssequence
+      (Sset _t'7
+        (Efield
+          (Ederef (Etempvar _att (tptr (Tstruct _index_attributes noattr)))
+            (Tstruct _index_attributes noattr)) _attrs
+          (tptr (Tstruct _attribute_list noattr))))
+      (Scall (Some _t'1)
+        (Evar _attr_list_length (Tfunction
+                                  (Tcons
+                                    (tptr (Tstruct _attribute_list noattr))
+                                    Tnil) tulong cc_default))
+        ((Etempvar _t'7 (tptr (Tstruct _attribute_list noattr))) :: nil)))
+    (Sset _numcols (Etempvar _t'1 tulong)))
+  (Ssequence
+    (Ssequence
+      (Ssequence
+        (Sset _t'5
+          (Efield
+            (Ederef (Etempvar _att (tptr (Tstruct _index_attributes noattr)))
+              (Tstruct _index_attributes noattr)) _attrs
+            (tptr (Tstruct _attribute_list noattr))))
+        (Ssequence
+          (Sset _t'6
+            (Efield
+              (Ederef
+                (Etempvar _att (tptr (Tstruct _index_attributes noattr)))
+                (Tstruct _index_attributes noattr)) _pk_attrs
+              (tptr (Tstruct _attribute_list noattr))))
+          (Scall (Some _t'2)
+            (Evar _index_of_pk_column (Tfunction
+                                        (Tcons
+                                          (tptr (Tstruct _attribute_list noattr))
+                                          (Tcons
+                                            (tptr (Tstruct _attribute_list noattr))
+                                            Tnil)) tint cc_default))
+            ((Etempvar _t'5 (tptr (Tstruct _attribute_list noattr))) ::
+             (Etempvar _t'6 (tptr (Tstruct _attribute_list noattr))) :: nil))))
+      (Sset _pk_num (Ecast (Etempvar _t'2 tint) tulong)))
+    (Ssequence
+      (Ssequence
+        (Sset _i (Ecast (Econst_int (Int.repr 0) tint) tulong))
+        (Sloop
+          (Ssequence
+            (Sifthenelse (Ebinop Olt (Etempvar _i tulong)
+                           (Etempvar _numrows tulong) tint)
+              Sskip
+              Sbreak)
+            (Ssequence
+              (Sset _ptr_to_row
+                (Ebinop Oadd (Etempvar _arr (tptr (Tunion _entry noattr)))
+                  (Ebinop Omul (Etempvar _i tulong)
+                    (Etempvar _numcols tulong) tulong)
+                  (tptr (Tunion _entry noattr))))
+              (Ssequence
+                (Sassign (Evar _key (Tunion _entry noattr))
+                  (Ederef
+                    (Ebinop Oadd
+                      (Etempvar _arr (tptr (Tunion _entry noattr)))
+                      (Ebinop Oadd
+                        (Ebinop Omul (Etempvar _i tulong)
+                          (Etempvar _numcols tulong) tulong)
+                        (Etempvar _pk_num tulong) tulong)
+                      (tptr (Tunion _entry noattr))) (Tunion _entry noattr)))
+                (Ssequence
+                  (Sset _t'4
+                    (Efield (Evar _key (Tunion _entry noattr)) _int_cont
+                      tulong))
+                  (Scall None
+                    (Evar _RL_PutRecord (Tfunction
+                                          (Tcons
+                                            (tptr (Tstruct _Cursor noattr))
+                                            (Tcons tulong
+                                              (Tcons (tptr tvoid) Tnil)))
+                                          tvoid cc_default))
+                    ((Etempvar _cur (tptr (Tstruct _Cursor noattr))) ::
+                     (Etempvar _t'4 tulong) ::
+                     (Etempvar _ptr_to_row (tptr tvoid)) :: nil))))))
+          (Sset _i
+            (Ebinop Oadd (Etempvar _i tulong) (Econst_int (Int.repr 1) tint)
+              tulong))))
+      (Ssequence
+        (Sset _t'3
+          (Efield
+            (Ederef (Etempvar _cur (tptr (Tstruct _Cursor noattr)))
+              (Tstruct _Cursor noattr)) _relation
+            (tptr (Tstruct _Relation noattr))))
+        (Sreturn (Some (Etempvar _t'3 (tptr (Tstruct _Relation noattr)))))))))
+|}.
+
+Definition v_data := {|
+  gvar_info := (tarray (Tunion _entry noattr) 8);
+  gvar_init := (Init_int64 (Int64.repr 1) ::
+                Init_addrof ___stringlit_27 (Ptrofs.repr 0) ::
+                Init_int64 (Int64.repr 2) ::
+                Init_addrof ___stringlit_26 (Ptrofs.repr 0) ::
+                Init_int64 (Int64.repr 3) ::
+                Init_addrof ___stringlit_25 (Ptrofs.repr 0) ::
+                Init_int64 (Int64.repr 4) ::
+                Init_addrof ___stringlit_24 (Ptrofs.repr 0) :: nil);
+  gvar_readonly := false;
+  gvar_volatile := false
+|}.
+
+Definition v_snd := {|
+  gvar_info := (Tstruct _attribute_list noattr);
+  gvar_init := (Init_addrof ___stringlit_28 (Ptrofs.repr 0) ::
+                Init_int32 (Int.repr 1) :: Init_space 4 ::
+                Init_int64 (Int64.repr 0) :: nil);
+  gvar_readonly := false;
+  gvar_volatile := false
+|}.
+
+Definition v_schema := {|
+  gvar_info := (Tstruct _attribute_list noattr);
+  gvar_init := (Init_addrof ___stringlit_29 (Ptrofs.repr 0) ::
+                Init_int32 (Int.repr 0) :: Init_space 4 ::
+                Init_addrof _snd (Ptrofs.repr 0) :: nil);
+  gvar_readonly := false;
+  gvar_volatile := false
+|}.
+
+Definition v_primary := {|
+  gvar_info := (Tstruct _attribute_list noattr);
+  gvar_init := (Init_addrof ___stringlit_29 (Ptrofs.repr 0) ::
+                Init_int32 (Int.repr 0) :: Init_space 4 ::
+                Init_int64 (Int64.repr 0) :: nil);
+  gvar_readonly := false;
+  gvar_volatile := false
+|}.
+
+Definition v_attrs := {|
+  gvar_info := (Tstruct _index_attributes noattr);
+  gvar_init := (Init_addrof _schema (Ptrofs.repr 0) ::
+                Init_addrof _primary (Ptrofs.repr 0) :: nil);
+  gvar_readonly := false;
+  gvar_volatile := false
+|}.
+
+Definition f_main := {|
+  fn_return := tint;
+  fn_callconv := cc_default;
+  fn_params := ((_argc, tint) :: (_argv, (tptr (tptr tschar))) :: nil);
+  fn_vars := nil;
+  fn_temps := ((_cur, (tptr (Tstruct _Cursor noattr))) ::
+               (_tree, (tptr (Tstruct _index_t noattr))) ::
+               (_bc1, (tptr (Tstruct _db_cursor_t noattr))) ::
+               (_bc2, (tptr (Tstruct _db_cursor_t noattr))) ::
+               (_t'4, (tptr (Tstruct _db_cursor_t noattr))) ::
+               (_t'3, (tptr (Tstruct _db_cursor_t noattr))) ::
+               (_t'2, (tptr (Tstruct _Relation noattr))) ::
+               (_t'1, (tptr (Tstruct _Cursor noattr))) ::
+               (_t'9,
+                (tptr (Tfunction
+                        (Tcons (tptr (Tstruct _index_t noattr)) Tnil)
+                        (tptr (Tstruct _db_cursor_t noattr)) cc_default))) ::
+               (_t'8,
+                (tptr (Tfunction
+                        (Tcons (tptr (Tstruct _index_t noattr)) Tnil)
+                        (tptr (Tstruct _db_cursor_t noattr)) cc_default))) ::
+               (_t'7,
+                (tptr (Tfunction
+                        (Tcons (tptr (Tstruct _db_cursor_t noattr)) Tnil)
+                        tint cc_default))) ::
+               (_t'6,
+                (tptr (Tfunction
+                        (Tcons (tptr (Tstruct _db_cursor_t noattr)) Tnil)
+                        tint cc_default))) ::
+               (_t'5,
+                (tptr (Tfunction
+                        (Tcons (tptr (Tstruct _db_cursor_t noattr)) Tnil)
+                        tint cc_default))) :: nil);
+  fn_body :=
+(Ssequence
+  (Ssequence
+    (Ssequence
+      (Scall (Some _t'1)
+        (Evar _create_relation (Tfunction
+                                 (Tcons
+                                   (tptr (Tstruct _index_attributes noattr))
+                                   Tnil) (tptr (Tstruct _Cursor noattr))
+                                 cc_default))
+        ((Eaddrof (Evar _attrs (Tstruct _index_attributes noattr))
+           (tptr (Tstruct _index_attributes noattr))) :: nil))
+      (Sset _cur (Etempvar _t'1 (tptr (Tstruct _Cursor noattr)))))
+    (Ssequence
+      (Ssequence
+        (Scall (Some _t'2)
+          (Evar _fill_relation (Tfunction
+                                 (Tcons (tptr (Tunion _entry noattr))
+                                   (Tcons (tptr (Tstruct _Cursor noattr))
+                                     (Tcons tulong
+                                       (Tcons
+                                         (tptr (Tstruct _index_attributes noattr))
+                                         Tnil))))
+                                 (tptr (Tstruct _Relation noattr))
+                                 cc_default))
+          ((Evar _data (tarray (Tunion _entry noattr) 8)) ::
+           (Etempvar _cur (tptr (Tstruct _Cursor noattr))) ::
+           (Econst_int (Int.repr 4) tint) ::
+           (Eaddrof (Evar _attrs (Tstruct _index_attributes noattr))
+             (tptr (Tstruct _index_attributes noattr))) :: nil))
+        (Sset _tree
+          (Ecast (Etempvar _t'2 (tptr (Tstruct _Relation noattr)))
+            (tptr (Tstruct _index_t noattr)))))
+      (Ssequence
+        (Ssequence
+          (Ssequence
+            (Sset _t'9
+              (Efield (Evar _btree_mtable (Tstruct _OrdIndexMtable noattr))
+                _create_cursor
+                (tptr (Tfunction
+                        (Tcons (tptr (Tstruct _index_t noattr)) Tnil)
+                        (tptr (Tstruct _db_cursor_t noattr)) cc_default))))
+            (Scall (Some _t'3)
+              (Etempvar _t'9 (tptr (Tfunction
+                                     (Tcons (tptr (Tstruct _index_t noattr))
+                                       Tnil)
+                                     (tptr (Tstruct _db_cursor_t noattr))
+                                     cc_default)))
+              ((Etempvar _tree (tptr (Tstruct _index_t noattr))) :: nil)))
+          (Sset _bc1
+            (Ecast (Etempvar _t'3 (tptr (Tstruct _db_cursor_t noattr)))
+              (tptr (Tstruct _db_cursor_t noattr)))))
+        (Ssequence
+          (Ssequence
+            (Ssequence
+              (Sset _t'8
+                (Efield (Evar _btree_mtable (Tstruct _OrdIndexMtable noattr))
+                  _create_cursor
+                  (tptr (Tfunction
+                          (Tcons (tptr (Tstruct _index_t noattr)) Tnil)
+                          (tptr (Tstruct _db_cursor_t noattr)) cc_default))))
+              (Scall (Some _t'4)
+                (Etempvar _t'8 (tptr (Tfunction
+                                       (Tcons
+                                         (tptr (Tstruct _index_t noattr))
+                                         Tnil)
+                                       (tptr (Tstruct _db_cursor_t noattr))
+                                       cc_default)))
+                ((Etempvar _tree (tptr (Tstruct _index_t noattr))) :: nil)))
+            (Sset _bc2
+              (Ecast (Etempvar _t'4 (tptr (Tstruct _db_cursor_t noattr)))
+                (tptr (Tstruct _db_cursor_t noattr)))))
+          (Ssequence
+            (Ssequence
+              (Sset _t'7
+                (Efield (Evar _btree_mtable (Tstruct _OrdIndexMtable noattr))
+                  _move_to_next
+                  (tptr (Tfunction
+                          (Tcons (tptr (Tstruct _db_cursor_t noattr)) Tnil)
+                          tint cc_default))))
+              (Scall None
+                (Etempvar _t'7 (tptr (Tfunction
+                                       (Tcons
+                                         (tptr (Tstruct _db_cursor_t noattr))
+                                         Tnil) tint cc_default)))
+                ((Etempvar _bc1 (tptr (Tstruct _db_cursor_t noattr))) :: nil)))
+            (Ssequence
+              (Ssequence
+                (Sset _t'6
+                  (Efield
+                    (Evar _btree_mtable (Tstruct _OrdIndexMtable noattr))
+                    _move_to_next
+                    (tptr (Tfunction
+                            (Tcons (tptr (Tstruct _db_cursor_t noattr)) Tnil)
+                            tint cc_default))))
+                (Scall None
+                  (Etempvar _t'6 (tptr (Tfunction
+                                         (Tcons
+                                           (tptr (Tstruct _db_cursor_t noattr))
+                                           Tnil) tint cc_default)))
+                  ((Etempvar _bc2 (tptr (Tstruct _db_cursor_t noattr))) ::
+                   nil)))
+              (Ssequence
+                (Sset _t'5
+                  (Efield
+                    (Evar _btree_mtable (Tstruct _OrdIndexMtable noattr))
+                    _move_to_next
+                    (tptr (Tfunction
+                            (Tcons (tptr (Tstruct _db_cursor_t noattr)) Tnil)
+                            tint cc_default))))
+                (Scall None
+                  (Etempvar _t'5 (tptr (Tfunction
+                                         (Tcons
+                                           (tptr (Tstruct _db_cursor_t noattr))
+                                           Tnil) tint cc_default)))
+                  ((Etempvar _bc2 (tptr (Tstruct _db_cursor_t noattr))) ::
+                   nil)))))))))
+  (Sreturn (Some (Econst_int (Int.repr 0) tint))))
+|}.
+
 Definition composites : list composite_definition :=
 (Composite ___sbuf Struct
    ((__base, (tptr tuchar)) :: (__size, tint) :: nil)
@@ -5006,6 +5903,54 @@ Definition composites : list composite_definition :=
     (__lb, (Tstruct ___sbuf noattr)) :: (__blksize, tint) ::
     (__offset, tlong) :: nil)
    noattr ::
+ Composite _attribute_list Struct
+   ((_id, (tptr tschar)) :: (_domain, tint) ::
+    (_next, (tptr (Tstruct _attribute_list noattr))) :: nil)
+   noattr ::
+ Composite _index_attributes Struct
+   ((_attrs, (tptr (Tstruct _attribute_list noattr))) ::
+    (_pk_attrs, (tptr (Tstruct _attribute_list noattr))) :: nil)
+   noattr ::
+ Composite _entry Union
+   ((_int_cont, tulong) :: (_str_cont, (tptr tschar)) :: nil)
+   noattr ::
+ Composite _BtreeCursor Struct
+   ((_btree, (tptr (Tstruct _Relation noattr))) ::
+    (_cur, (tptr (Tstruct _Cursor noattr))) :: nil)
+   noattr ::
+ Composite _OrdIndexMtable Struct
+   ((_create_index,
+     (tptr (Tfunction Tnil (tptr (Tstruct _db_cursor_t noattr))
+             {|cc_vararg:=false; cc_unproto:=true; cc_structret:=false|}))) ::
+    (_create_cursor,
+     (tptr (Tfunction (Tcons (tptr (Tstruct _index_t noattr)) Tnil)
+             (tptr (Tstruct _db_cursor_t noattr)) cc_default))) ::
+    (_cardinality,
+     (tptr (Tfunction (Tcons (tptr (Tstruct _db_cursor_t noattr)) Tnil)
+             tulong cc_default))) ::
+    (_move_to_next,
+     (tptr (Tfunction (Tcons (tptr (Tstruct _db_cursor_t noattr)) Tnil) tint
+             cc_default))) ::
+    (_move_to_first,
+     (tptr (Tfunction (Tcons (tptr (Tstruct _db_cursor_t noattr)) Tnil) tint
+             cc_default))) ::
+    (_go_to_key,
+     (tptr (Tfunction
+             (Tcons (tptr (Tstruct _db_cursor_t noattr))
+               (Tcons (tptr (Tstruct _key_t noattr)) Tnil)) tint cc_default))) ::
+    (_cursor_has_next,
+     (tptr (Tfunction (Tcons (tptr (Tstruct _db_cursor_t noattr)) Tnil) tint
+             cc_default))) ::
+    (_put_record,
+     (tptr (Tfunction
+             (Tcons (tptr (Tstruct _db_cursor_t noattr))
+               (Tcons (tptr (Tstruct _key_t noattr))
+                 (Tcons (tptr (Tstruct _value_t noattr)) Tnil))) tvoid
+             cc_default))) ::
+    (_get_record,
+     (tptr (Tfunction (Tcons (tptr (Tstruct _db_cursor_t noattr)) Tnil)
+             (tptr (Tstruct _value_t noattr)) cc_default))) :: nil)
+   noattr ::
  Composite _Relation Struct
    ((_root, (tptr (Tstruct _BtNode noattr))) :: (_numRecords, tulong) ::
     (_depth, tint) :: nil)
@@ -5031,6 +5976,9 @@ Definition composites : list composite_definition :=
 Definition global_definitions : list (ident * globdef fundef type) :=
 ((___stringlit_14, Gvar v___stringlit_14) ::
  (___stringlit_4, Gvar v___stringlit_4) ::
+ (___stringlit_23, Gvar v___stringlit_23) ::
+ (___stringlit_29, Gvar v___stringlit_29) ::
+ (___stringlit_26, Gvar v___stringlit_26) ::
  (___stringlit_5, Gvar v___stringlit_5) ::
  (___stringlit_15, Gvar v___stringlit_15) ::
  (___stringlit_18, Gvar v___stringlit_18) ::
@@ -5038,19 +5986,23 @@ Definition global_definitions : list (ident * globdef fundef type) :=
  (___stringlit_12, Gvar v___stringlit_12) ::
  (___stringlit_21, Gvar v___stringlit_21) ::
  (___stringlit_8, Gvar v___stringlit_8) ::
+ (___stringlit_25, Gvar v___stringlit_25) ::
  (___stringlit_16, Gvar v___stringlit_16) ::
  (___stringlit_17, Gvar v___stringlit_17) ::
  (___stringlit_3, Gvar v___stringlit_3) ::
+ (___stringlit_27, Gvar v___stringlit_27) ::
  (___stringlit_1, Gvar v___stringlit_1) ::
  (___stringlit_6, Gvar v___stringlit_6) ::
+ (___stringlit_24, Gvar v___stringlit_24) ::
  (___stringlit_19, Gvar v___stringlit_19) ::
  (___stringlit_11, Gvar v___stringlit_11) ::
  (___stringlit_22, Gvar v___stringlit_22) ::
- (___stringlit_2, Gvar v___stringlit_2) ::
  (___stringlit_7, Gvar v___stringlit_7) ::
+ (___stringlit_28, Gvar v___stringlit_28) ::
  (___stringlit_9, Gvar v___stringlit_9) ::
  (___stringlit_13, Gvar v___stringlit_13) ::
  (___stringlit_20, Gvar v___stringlit_20) ::
+ (___stringlit_2, Gvar v___stringlit_2) ::
  (___builtin_bswap,
    Gfun(External (EF_builtin "__builtin_bswap"
                    (mksignature (AST.Tint :: nil) (Some AST.Tint) cc_default))
@@ -5295,9 +6247,7 @@ Definition global_definitions : list (ident * globdef fundef type) :=
                      {|cc_vararg:=true; cc_unproto:=false; cc_structret:=false|}))
      (Tcons tint Tnil) tvoid
      {|cc_vararg:=true; cc_unproto:=false; cc_structret:=false|})) ::
- (_abort,
-   Gfun(External (EF_external "abort" (mksignature nil None cc_default)) Tnil
-     tvoid cc_default)) :: (___stderrp, Gvar v___stderrp) ::
+ (___stderrp, Gvar v___stderrp) ::
  (_fprintf,
    Gfun(External (EF_external "fprintf"
                    (mksignature (AST.Tlong :: AST.Tlong :: nil)
@@ -5305,19 +6255,11 @@ Definition global_definitions : list (ident * globdef fundef type) :=
                      {|cc_vararg:=true; cc_unproto:=false; cc_structret:=false|}))
      (Tcons (tptr (Tstruct ___sFILE noattr)) (Tcons (tptr tschar) Tnil)) tint
      {|cc_vararg:=true; cc_unproto:=false; cc_structret:=false|})) ::
- (_printf,
-   Gfun(External (EF_external "printf"
-                   (mksignature (AST.Tlong :: nil) (Some AST.Tint)
-                     {|cc_vararg:=true; cc_unproto:=false; cc_structret:=false|}))
-     (Tcons (tptr tschar) Tnil) tint
-     {|cc_vararg:=true; cc_unproto:=false; cc_structret:=false|})) ::
- (_free, Gfun(External EF_free (Tcons (tptr tvoid) Tnil) tvoid cc_default)) ::
- (_malloc,
-   Gfun(External EF_malloc (Tcons tulong Tnil) (tptr tvoid) cc_default)) ::
- (_exit,
-   Gfun(External (EF_external "exit"
-                   (mksignature (AST.Tint :: nil) None cc_default))
-     (Tcons tint Tnil) tvoid cc_default)) ::
+ (_strcmp,
+   Gfun(External (EF_external "strcmp"
+                   (mksignature (AST.Tlong :: AST.Tlong :: nil)
+                     (Some AST.Tint) cc_default))
+     (Tcons (tptr tschar) (Tcons (tptr tschar) Tnil)) tint cc_default)) ::
  (_surely_malloc, Gfun(Internal f_surely_malloc)) ::
  (_entryIndex, Gfun(Internal f_entryIndex)) ::
  (_currNode, Gfun(Internal f_currNode)) ::
@@ -5359,35 +6301,73 @@ Definition global_definitions : list (ident * globdef fundef type) :=
  (_moveToLast, Gfun(Internal f_moveToLast)) ::
  (_handleDeleteBtree, Gfun(Internal f_handleDeleteBtree)) ::
  (_printTree, Gfun(Internal f_printTree)) ::
- (_printCursor, Gfun(Internal f_printCursor)) :: nil).
+ (_printCursor, Gfun(Internal f_printCursor)) ::
+ (_malloc,
+   Gfun(External EF_malloc (Tcons tulong Tnil) (tptr tvoid) cc_default)) ::
+ (_free, Gfun(External EF_free (Tcons (tptr tvoid) Tnil) tvoid cc_default)) ::
+ (_exit,
+   Gfun(External (EF_external "exit"
+                   (mksignature (AST.Tint :: nil) None cc_default))
+     (Tcons tint Tnil) tvoid cc_default)) ::
+ (_abort,
+   Gfun(External (EF_external "abort" (mksignature nil None cc_default)) Tnil
+     tvoid cc_default)) ::
+ (_printf,
+   Gfun(External (EF_external "printf"
+                   (mksignature (AST.Tlong :: nil) (Some AST.Tint)
+                     {|cc_vararg:=true; cc_unproto:=false; cc_structret:=false|}))
+     (Tcons (tptr tschar) Tnil) tint
+     {|cc_vararg:=true; cc_unproto:=false; cc_structret:=false|})) ::
+ (_btree_create_index, Gfun(Internal f_btree_create_index)) ::
+ (_btree_create_cursor, Gfun(Internal f_btree_create_cursor)) ::
+ (_btree_cardinality, Gfun(Internal f_btree_cardinality)) ::
+ (_btree_move_to_next, Gfun(Internal f_btree_move_to_next)) ::
+ (_btree_move_to_first, Gfun(Internal f_btree_move_to_first)) ::
+ (_btree_go_to_key, Gfun(Internal f_btree_go_to_key)) ::
+ (_btree_cursor_has_next, Gfun(Internal f_btree_cursor_has_next)) ::
+ (_btree_put_record, Gfun(Internal f_btree_put_record)) ::
+ (_btree_get_record, Gfun(Internal f_btree_get_record)) ::
+ (_btree_mtable, Gvar v_btree_mtable) ::
+ (_attr_list_length, Gfun(Internal f_attr_list_length)) ::
+ (_index_of_pk_column, Gfun(Internal f_index_of_pk_column)) ::
+ (_create_relation, Gfun(Internal f_create_relation)) ::
+ (_fill_relation, Gfun(Internal f_fill_relation)) :: (_data, Gvar v_data) ::
+ (_snd, Gvar v_snd) :: (_schema, Gvar v_schema) ::
+ (_primary, Gvar v_primary) :: (_attrs, Gvar v_attrs) ::
+ (_main, Gfun(Internal f_main)) :: nil).
 
 Definition public_idents : list ident :=
-(_RL_PrintCursor :: _RL_PrintTree :: _RL_NumRecords :: _RL_IsEmpty ::
+(_main :: _attrs :: _primary :: _schema :: _snd :: _data :: _fill_relation ::
+ _create_relation :: _index_of_pk_column :: _attr_list_length ::
+ _btree_mtable :: _btree_get_record :: _btree_put_record ::
+ _btree_cursor_has_next :: _btree_go_to_key :: _btree_move_to_first ::
+ _btree_move_to_next :: _btree_cardinality :: _btree_create_cursor ::
+ _btree_create_index :: _printf :: _abort :: _exit :: _free :: _malloc ::
+ _RL_PrintCursor :: _RL_PrintTree :: _RL_NumRecords :: _RL_IsEmpty ::
  _RL_MoveToPreviousNotFirst :: _RL_MoveToNextValid :: _RL_MoveToPrevious ::
  _RL_MoveToNext :: _firstpointer :: _lastpointer :: _RL_MoveToFirst ::
  _RL_DeleteRecord :: _RL_MoveToKey :: _RL_GetKey :: _RL_GetRecord ::
  _AscendToParent :: _RL_PutRecord :: _RL_CursorIsValid :: _RL_FreeCursor ::
  _RL_NewCursor :: _RL_DeleteRelation :: _RL_NewRelation :: _isFirst ::
- _isValid :: _currNode :: _entryIndex :: _surely_malloc :: _exit ::
- _malloc :: _free :: _printf :: _fprintf :: ___stderrp :: _abort ::
- ___builtin_debug :: ___builtin_nop :: ___builtin_write32_reversed ::
- ___builtin_write16_reversed :: ___builtin_read32_reversed ::
- ___builtin_read16_reversed :: ___builtin_fnmsub :: ___builtin_fnmadd ::
- ___builtin_fmsub :: ___builtin_fmadd :: ___builtin_fmin ::
- ___builtin_fmax :: ___builtin_ctzll :: ___builtin_ctzl :: ___builtin_ctz ::
- ___builtin_clzll :: ___builtin_clzl :: ___builtin_clz ::
- ___builtin_bswap64 :: ___compcert_i64_umulh :: ___compcert_i64_smulh ::
- ___compcert_i64_sar :: ___compcert_i64_shr :: ___compcert_i64_shl ::
- ___compcert_i64_umod :: ___compcert_i64_smod :: ___compcert_i64_udiv ::
- ___compcert_i64_sdiv :: ___compcert_i64_utof :: ___compcert_i64_stof ::
- ___compcert_i64_utod :: ___compcert_i64_stod :: ___compcert_i64_dtou ::
- ___compcert_i64_dtos :: ___compcert_va_composite ::
- ___compcert_va_float64 :: ___compcert_va_int64 :: ___compcert_va_int32 ::
- ___builtin_va_end :: ___builtin_va_copy :: ___builtin_va_arg ::
- ___builtin_va_start :: ___builtin_membar :: ___builtin_annot_intval ::
- ___builtin_annot :: ___builtin_memcpy_aligned :: ___builtin_fsqrt ::
- ___builtin_fabs :: ___builtin_bswap16 :: ___builtin_bswap32 ::
- ___builtin_bswap :: nil).
+ _isValid :: _currNode :: _entryIndex :: _surely_malloc :: _strcmp ::
+ _fprintf :: ___stderrp :: ___builtin_debug :: ___builtin_nop ::
+ ___builtin_write32_reversed :: ___builtin_write16_reversed ::
+ ___builtin_read32_reversed :: ___builtin_read16_reversed ::
+ ___builtin_fnmsub :: ___builtin_fnmadd :: ___builtin_fmsub ::
+ ___builtin_fmadd :: ___builtin_fmin :: ___builtin_fmax ::
+ ___builtin_ctzll :: ___builtin_ctzl :: ___builtin_ctz :: ___builtin_clzll ::
+ ___builtin_clzl :: ___builtin_clz :: ___builtin_bswap64 ::
+ ___compcert_i64_umulh :: ___compcert_i64_smulh :: ___compcert_i64_sar ::
+ ___compcert_i64_shr :: ___compcert_i64_shl :: ___compcert_i64_umod ::
+ ___compcert_i64_smod :: ___compcert_i64_udiv :: ___compcert_i64_sdiv ::
+ ___compcert_i64_utof :: ___compcert_i64_stof :: ___compcert_i64_utod ::
+ ___compcert_i64_stod :: ___compcert_i64_dtou :: ___compcert_i64_dtos ::
+ ___compcert_va_composite :: ___compcert_va_float64 ::
+ ___compcert_va_int64 :: ___compcert_va_int32 :: ___builtin_va_end ::
+ ___builtin_va_copy :: ___builtin_va_arg :: ___builtin_va_start ::
+ ___builtin_membar :: ___builtin_annot_intval :: ___builtin_annot ::
+ ___builtin_memcpy_aligned :: ___builtin_fsqrt :: ___builtin_fabs ::
+ ___builtin_bswap16 :: ___builtin_bswap32 :: ___builtin_bswap :: nil).
 
 Definition prog : Clight.program := 
   mkprogram composites global_definitions public_idents _main Logic.I.
