verif/indices/db_cursor.v
@@ -1,0 +1,148 @@
+Require Import VST.floyd.proofauto.
+Require Import VST.floyd.library.
+Require Import indices.ordered_interface.
+Require Import indices.spec_BtreeIndexASI.
+Require Import indices.btree_instance.
+Require Import VST.msl.wand_frame.
+Require Import VST.msl.iter_sepcon.
+Require Import VST.floyd.reassoc_seq.
+Require Import VST.floyd.field_at_wand.
+Module DB_Cursor.
+
+Import OrderedIndex.
+
+Record db_cursor (oi: OrderedIndex.index) :=
+{ 
+  db_cursor_type: type;
+  db_key_type: type;
+  db_value_type: type;
+  db_index_type:type;
+
+  db_entry_rep: val -> val -> mpred;
+  db_cursor_rep: oi.(cursor) -> val-> val-> val-> mpred
+}.
+
+(* =================  FUNSPECS (VOID PTRS + DB CURSOR) =============== *)
+
+Definition create_index_spec_vp 
+  (oi: OrderedIndex.index) (db: db_cursor oi): funspec :=
+  WITH u:unit, gv: globals
+  PRE [ ]
+    PROP ()
+    PARAMS() GLOBALS(gv)
+    SEP (mem_mgr gv)
+  POST [tptr (db_cursor_type oi db) ]
+    EX m: oi.(t), EX pr: val,
+    PROP (oi.(create_index) m)
+    LOCAL(temp ret_temp pr)
+    SEP (mem_mgr gv; oi.(t_repr) m pr). 
+
+Definition put_record_spec_vp 
+  (oi: OrderedIndex.index) (db: db_cursor oi): funspec :=
+   WITH cur: oi.(cursor), cur_ptr:val, key:oi.(key), pkey: val, recordptr:val, record:oi.(value), gv: globals,
+            e_ptr: val, t_ptr: val, ws_ptr: val
+  PRE [ tptr (db_cursor_type oi db), tptr (db_key_type oi db), tptr (db_value_type oi db)]
+    PROP(oi.(put_record_props) cur)
+    PARAMS(ws_ptr; e_ptr; recordptr) GLOBALS(gv)
+    SEP(mem_mgr gv; oi.(value_repr) record recordptr * 
+          (db_cursor_rep oi db) cur t_ptr cur_ptr ws_ptr * 
+          (db_entry_rep oi db) e_ptr (oi.(key_val) key))
+  POST [tvoid]
+    EX newc: oi.(cursor), 
+    PROP(oi.(put_record) cur key record recordptr newc)
+    LOCAL()
+    SEP(mem_mgr gv; (db_cursor_rep oi db) newc t_ptr cur_ptr ws_ptr * 
+          (db_entry_rep oi db) e_ptr (oi.(key_val) key)).
+
+Definition go_to_key_spec_vp
+  (oi: OrderedIndex.index) (db: db_cursor oi): funspec :=
+  WITH cur:oi.(cursor), cur_ptr:val, key:oi.(key), e_ptr: val, t_ptr: val, ws_ptr: val
+  PRE [ tptr (db_cursor_type oi db), tptr (db_key_type oi db) ]
+    PROP(oi.(go_to_key_props) cur)
+    PARAMS(ws_ptr; e_ptr) GLOBALS()
+    SEP((db_cursor_rep oi db) cur t_ptr cur_ptr ws_ptr * 
+      (db_entry_rep oi db) e_ptr (oi.(key_val) key))
+  POST [tint]
+    PROP()
+    LOCAL(temp ret_temp (Val.of_bool (oi.(cursor_has_next) (oi.(go_to_key) cur key))))
+    SEP((db_cursor_rep oi db) (oi.(go_to_key) cur key) t_ptr cur_ptr ws_ptr * 
+      (db_entry_rep oi db) e_ptr (oi.(key_val) key)).
+
+Definition cardinality_spec_vp
+  (oi: OrderedIndex.index) (db: db_cursor oi): funspec :=
+  WITH cur_ptr: val, cur: oi.(cursor), t_ptr:val, ws_ptr:val
+  PRE [tptr (db_cursor_type oi db)]
+    PROP()
+    PARAMS(ws_ptr) GLOBALS()
+    SEP((db_cursor_rep oi db) cur t_ptr cur_ptr ws_ptr)
+  POST [size_t]
+    PROP()
+    LOCAL(temp ret_temp (Vptrofs (Ptrofs.repr (oi.(cardinality) cur))))
+    SEP((db_cursor_rep oi db) cur t_ptr cur_ptr ws_ptr).
+
+Definition cursor_has_next_spec_vp
+  (oi: OrderedIndex.index) (db: db_cursor oi): funspec :=
+  WITH cur:oi.(cursor), cur_ptr:val, t_ptr: val, ws_ptr:val
+  PRE [ tptr (db_cursor_type oi db) ]
+    PROP(oi.(cursor_has_next_props) cur)
+    PARAMS(ws_ptr) GLOBALS()
+    SEP((db_cursor_rep oi db) cur t_ptr cur_ptr ws_ptr)
+  POST [tint]
+    PROP()
+    LOCAL(temp ret_temp (Val.of_bool (oi.(cursor_has_next) cur)))
+    SEP((db_cursor_rep oi db) cur t_ptr cur_ptr ws_ptr).
+
+Definition move_to_next_spec_vp 
+  (oi: OrderedIndex.index) (db: db_cursor oi): funspec :=
+  WITH cur_ptr: val, cur: oi.(cursor), t_ptr: val, ws_ptr:val
+  PRE [ tptr (db_cursor_type oi db)]
+    PROP(oi.(move_to_next_props) cur)
+    PARAMS(ws_ptr) GLOBALS()
+    SEP((db_cursor_rep oi db) cur t_ptr cur_ptr ws_ptr)
+  POST [tint]
+    PROP()
+    LOCAL(temp ret_temp (Val.of_bool (oi.(cursor_has_next) (oi.(move_to_next) cur))))
+    SEP((db_cursor_rep oi db) (oi.(move_to_next) cur) t_ptr cur_ptr ws_ptr).
+
+Definition move_to_first_spec_vp
+  (oi: OrderedIndex.index) (db: db_cursor oi): funspec :=
+  WITH gv: globals, cur_ptr: val, cur: oi.(cursor), t_ptr: val, ws_ptr: val
+  PRE [ tptr (db_cursor_type oi db)]
+    PROP(oi.(move_to_first_props) cur)
+    PARAMS(ws_ptr) GLOBALS()
+    SEP(mem_mgr gv; (db_cursor_rep oi db) cur t_ptr cur_ptr ws_ptr)
+  POST [tint]
+    PROP()
+    LOCAL(temp ret_temp (Val.of_bool (oi.(cursor_has_next) (oi.(move_to_first) cur))))
+    SEP(mem_mgr gv; (db_cursor_rep oi db) (oi.(move_to_first) cur) t_ptr cur_ptr ws_ptr).
+
+Definition get_record_spec_vp
+  (oi: OrderedIndex.index) (db: db_cursor oi): funspec :=
+  WITH cur_ptr: val, cur: oi.(cursor), t_ptr: val, ws_ptr: val
+  PRE [tptr (db_cursor_type oi db)]
+    PROP(oi.(get_record_props) cur)
+    PARAMS(ws_ptr) GLOBALS()
+    SEP((db_cursor_rep oi db) cur t_ptr cur_ptr ws_ptr)
+  POST [tptr (db_value_type oi db)]
+    EX newc,
+    PROP()
+    LOCAL(temp ret_temp (oi.(get_record) cur))
+    SEP((db_cursor_rep oi db) newc t_ptr cur_ptr ws_ptr).
+
+(* magic wand to allow for multiple cursors
+on one data structure *)
+Definition create_cursor_spec_vp
+  (oi: OrderedIndex.index) (db: db_cursor oi): funspec :=
+  WITH r: oi.(t), gv: globals, t_ptr: val
+  PRE [tptr (db_index_type oi db)]
+    PROP(oi.(create_cursor_props) r t_ptr)
+    PARAMS(t_ptr) GLOBALS(gv)
+    SEP(mem_mgr gv; oi.(t_repr) r t_ptr)
+  POST [tptr (db_cursor_type oi db)]
+    EX cur_ptr ws_ptr,
+    PROP()
+    LOCAL(temp ret_temp ws_ptr)
+    SEP(mem_mgr gv; oi.(t_repr) r t_ptr; 
+      (oi.(t_repr) r t_ptr -* (db_cursor_rep oi db) (oi.(create_cursor) r) t_ptr cur_ptr ws_ptr)).
+
+End DB_Cursor.
