verif/indices/definitions.v
@@ -6,3 +6,4 @@ Definition nullV: V := exist _ nullval mapsto_memory_block.is_pointer_or_null_nu
 Definition V_repr: V -> val := @proj1_sig _ _.
 Definition maybe {A: Type} (o: option A) (default: A) :=
   match o with Some a => a | None => default end.
+
